src/coq/Transformations/UndefTests.v
@@ -12,8 +12,8 @@ Definition undef_test0_block : block dtyp :=
   {|
     blk_id := (Anon 0%Z);
     blk_phis := [];
-    blk_code := [(IId (Name "r"), (INSTR_Op (OP_IBinop (Mul false false) (DTYPE_I 64%Z) EXP_Undef EXP_Undef)))];
-    blk_term := (IVoid 0%Z, TERM_Ret ((DTYPE_I 64%Z), (EXP_Ident (ID_Local (Name "r")))));
+    blk_code := [(IId (Name "r"), (INSTR_Op (OP_IBinop (Mul false false) (DTYPE_I 64%N) EXP_Undef EXP_Undef)))];
+    blk_term := TERM_Ret ((DTYPE_I 64%N), (EXP_Ident (ID_Local (Name "r"))));
     blk_comments := None
   |}.
 
@@ -22,7 +22,7 @@ Definition undef_test0_block_refine : block dtyp :=
     blk_id := (Anon 0%Z);
     blk_phis := [];
     blk_code := [];
-    blk_term := (IVoid 0%Z, TERM_Ret ((DTYPE_I 64%Z), (EXP_Undef)));
+    blk_term := TERM_Ret ((DTYPE_I 64%N), (EXP_Undef));
     blk_comments := None
   |}.
 
@@ -30,8 +30,8 @@ Definition undef_test1_block : block dtyp
   := {|
       blk_id := (Anon 0%Z);
       blk_phis := [];
-      blk_code := [(IId (Name "r"), (INSTR_Op (OP_IBinop (Mul false false) (DTYPE_I 64%Z) (EXP_Integer 3%Z) EXP_Undef)))];
-      blk_term := (IVoid 0%Z, TERM_Ret ((DTYPE_I 64%Z), (EXP_Ident (ID_Local (Name "r")))));
+      blk_code := [(IId (Name "r"), (INSTR_Op (OP_IBinop (Mul false false) (DTYPE_I 64%N) (EXP_Integer 3%Z) EXP_Undef)))];
+      blk_term := TERM_Ret ((DTYPE_I 64%N), (EXP_Ident (ID_Local (Name "r"))));
       blk_comments := None
     |}.
 
@@ -41,8 +41,8 @@ Definition undef_test2_block : block dtyp
   := {|
       blk_id := (Anon 0%Z);
       blk_phis := [];
-      blk_code := [(IId (Name "r"), (INSTR_Op (OP_IBinop (Mul false false) (DTYPE_I 64%Z) EXP_Undef (EXP_Integer 3%Z))))];
-      blk_term := (IVoid 0%Z, TERM_Ret ((DTYPE_I 64%Z), (EXP_Ident (ID_Local (Name "r")))));
+      blk_code := [(IId (Name "r"), (INSTR_Op (OP_IBinop (Mul false false) (DTYPE_I 64%N) EXP_Undef (EXP_Integer 3%Z))))];
+      blk_term := TERM_Ret ((DTYPE_I 64%N), (EXP_Ident (ID_Local (Name "r"))));
       blk_comments := None
     |}.
 
@@ -52,8 +52,8 @@ Definition undef_test3_block : block dtyp
   := {|
       blk_id := (Anon 0%Z);
       blk_phis := [];
-      blk_code := [(IId (Name "r"), (INSTR_Op (OP_IBinop (Mul false false) (DTYPE_I 64%Z) EXP_Undef (EXP_Integer 6%Z))))];
-      blk_term := (IVoid 0%Z, TERM_Ret ((DTYPE_I 64%Z), (EXP_Ident (ID_Local (Name "r")))));
+      blk_code := [(IId (Name "r"), (INSTR_Op (OP_IBinop (Mul false false) (DTYPE_I 64%N) EXP_Undef (EXP_Integer 6%Z))))];
+      blk_term := TERM_Ret ((DTYPE_I 64%N), (EXP_Ident (ID_Local (Name "r"))));
       blk_comments := None
     |}.
 
@@ -62,7 +62,7 @@ Definition undef_test3_block_refine : block dtyp
       blk_id := (Anon 0%Z);
       blk_phis := [];
       blk_code := [];
-      blk_term := (IVoid 0%Z, TERM_Ret ((DTYPE_I 64%Z), (EXP_Integer 0%Z)));
+      blk_term := TERM_Ret ((DTYPE_I 64%N), (EXP_Integer 0%Z));
       blk_comments := None
     |}.
 
@@ -71,8 +71,8 @@ Definition undef_test4_block : block dtyp
   := {|
       blk_id := (Anon 0%Z);
       blk_phis := [];
-      blk_code := [(IId (Name "r"), (INSTR_Op (OP_IBinop (Mul false false) (DTYPE_I 64%Z) (EXP_Integer 6%Z) EXP_Undef)))];
-      blk_term := (IVoid 0%Z, TERM_Ret ((DTYPE_I 64%Z), (EXP_Ident (ID_Local (Name "r")))));
+      blk_code := [(IId (Name "r"), (INSTR_Op (OP_IBinop (Mul false false) (DTYPE_I 64%N) (EXP_Integer 6%Z) EXP_Undef)))];
+      blk_term := TERM_Ret ((DTYPE_I 64%N), (EXP_Ident (ID_Local (Name "r"))));
       blk_comments := None
     |}.
 
@@ -82,8 +82,8 @@ Definition undef_test5_block : block dtyp
   := {|
       blk_id := (Anon 0%Z);
       blk_phis := [];
-      blk_code := [(IId (Name "r"), (INSTR_Op (OP_IBinop And (DTYPE_I 64%Z) EXP_Undef EXP_Undef)))];
-      blk_term := (IVoid 0%Z, TERM_Ret ((DTYPE_I 64%Z), (EXP_Ident (ID_Local (Name "r")))));
+      blk_code := [(IId (Name "r"), (INSTR_Op (OP_IBinop And (DTYPE_I 64%N) EXP_Undef EXP_Undef)))];
+      blk_term := TERM_Ret ((DTYPE_I 64%N), (EXP_Ident (ID_Local (Name "r"))));
       blk_comments := None
     |}.
 
@@ -93,8 +93,8 @@ Definition undef_test6_block : block dtyp
   := {|
       blk_id := (Anon 0%Z);
       blk_phis := [];
-      blk_code := [(IId (Name "r"), (INSTR_Op (OP_IBinop Or (DTYPE_I 64%Z) EXP_Undef EXP_Undef)))];
-      blk_term := (IVoid 0%Z, TERM_Ret ((DTYPE_I 64%Z), (EXP_Ident (ID_Local (Name "r")))));
+      blk_code := [(IId (Name "r"), (INSTR_Op (OP_IBinop Or (DTYPE_I 64%N) EXP_Undef EXP_Undef)))];
+      blk_term := TERM_Ret ((DTYPE_I 64%N), (EXP_Ident (ID_Local (Name "r"))));
       blk_comments := None
     |}.
 
@@ -104,8 +104,8 @@ Definition undef_test7_block : block dtyp
   := {|
       blk_id := (Anon 0%Z);
       blk_phis := [];
-      blk_code := [(IId (Name "r"), (INSTR_Op (OP_IBinop (UDiv false) (DTYPE_I 64%Z) EXP_Undef (EXP_Integer 1%Z))))];
-      blk_term := (IVoid 0%Z, TERM_Ret ((DTYPE_I 64%Z), (EXP_Ident (ID_Local (Name "r")))));
+      blk_code := [(IId (Name "r"), (INSTR_Op (OP_IBinop (UDiv false) (DTYPE_I 64%N) EXP_Undef (EXP_Integer 1%Z))))];
+      blk_term := TERM_Ret ((DTYPE_I 64%N), (EXP_Ident (ID_Local (Name "r"))));
       blk_comments := None
     |}.
 
@@ -115,8 +115,8 @@ Definition undef_test8_block : block dtyp
   := {|
       blk_id := (Anon 0%Z);
       blk_phis := [];
-      blk_code := [(IId (Name "r"), (INSTR_Op (OP_IBinop (SDiv false) (DTYPE_I 64%Z) EXP_Undef (EXP_Integer 1%Z))))];
-      blk_term := (IVoid 0%Z, TERM_Ret ((DTYPE_I 64%Z), (EXP_Ident (ID_Local (Name "r")))));
+      blk_code := [(IId (Name "r"), (INSTR_Op (OP_IBinop (SDiv false) (DTYPE_I 64%N) EXP_Undef (EXP_Integer 1%Z))))];
+      blk_term := TERM_Ret ((DTYPE_I 64%N), (EXP_Ident (ID_Local (Name "r"))));
       blk_comments := None
     |}.
 
@@ -126,8 +126,8 @@ Definition undef_test9_block : block dtyp
   := {|
       blk_id := (Anon 0%Z);
       blk_phis := [];
-      blk_code := [(IId (Name "r"), (INSTR_Op (OP_IBinop URem (DTYPE_I 64%Z) EXP_Undef (EXP_Integer 1%Z))))];
-      blk_term := (IVoid 0%Z, TERM_Ret ((DTYPE_I 64%Z), (EXP_Ident (ID_Local (Name "r")))));
+      blk_code := [(IId (Name "r"), (INSTR_Op (OP_IBinop URem (DTYPE_I 64%N) EXP_Undef (EXP_Integer 1%Z))))];
+      blk_term := TERM_Ret ((DTYPE_I 64%N), (EXP_Ident (ID_Local (Name "r"))));
       blk_comments := None
     |}.
 
@@ -137,8 +137,8 @@ Definition undef_test10_block : block dtyp
   := {|
       blk_id := (Anon 0%Z);
       blk_phis := [];
-      blk_code := [(IId (Name "r"), (INSTR_Op (OP_IBinop SRem (DTYPE_I 64%Z) EXP_Undef (EXP_Integer 1%Z))))];
-      blk_term := (IVoid 0%Z, TERM_Ret ((DTYPE_I 64%Z), (EXP_Ident (ID_Local (Name "r")))));
+      blk_code := [(IId (Name "r"), (INSTR_Op (OP_IBinop SRem (DTYPE_I 64%N) EXP_Undef (EXP_Integer 1%Z))))];
+      blk_term := TERM_Ret ((DTYPE_I 64%N), (EXP_Ident (ID_Local (Name "r"))));
       blk_comments := None
     |}.
 
@@ -148,8 +148,8 @@ Definition undef_test11_block : block dtyp
   := {|
       blk_id := (Anon 0%Z);
       blk_phis := [];
-      blk_code := [(IId (Name "r"), (INSTR_Op (OP_IBinop (Shl false false) (DTYPE_I 64%Z) EXP_Undef EXP_Undef)))];
-      blk_term := (IVoid 0%Z, TERM_Ret ((DTYPE_I 64%Z), (EXP_Ident (ID_Local (Name "r")))));
+      blk_code := [(IId (Name "r"), (INSTR_Op (OP_IBinop (Shl false false) (DTYPE_I 64%N) EXP_Undef EXP_Undef)))];
+      blk_term := TERM_Ret ((DTYPE_I 64%N), (EXP_Ident (ID_Local (Name "r"))));
       blk_comments := None
     |}.
 
@@ -157,8 +157,8 @@ Definition undef_test11b_block : block dtyp
   := {|
       blk_id := (Anon 0%Z);
       blk_phis := [];
-      blk_code := [(IId (Name "r"), (INSTR_Op (OP_IBinop (Shl false false) (DTYPE_I 64%Z) (EXP_Ident (ID_Local (Name "a"))) EXP_Undef)))];
-      blk_term := (IVoid 0%Z, TERM_Ret ((DTYPE_I 64%Z), (EXP_Ident (ID_Local (Name "r")))));
+      blk_code := [(IId (Name "r"), (INSTR_Op (OP_IBinop (Shl false false) (DTYPE_I 64%N) (EXP_Ident (ID_Local (Name "a"))) EXP_Undef)))];
+      blk_term := TERM_Ret ((DTYPE_I 64%N), (EXP_Ident (ID_Local (Name "r"))));
       blk_comments := None
     |}.
 
@@ -166,8 +166,8 @@ Definition undef_test12_block : block dtyp
   := {|
       blk_id := (Anon 0%Z);
       blk_phis := [];
-      blk_code := [(IId (Name "r"), (INSTR_Op (OP_IBinop (AShr false) (DTYPE_I 64%Z) EXP_Undef EXP_Undef)))];
-      blk_term := (IVoid 0%Z, TERM_Ret ((DTYPE_I 64%Z), (EXP_Ident (ID_Local (Name "r")))));
+      blk_code := [(IId (Name "r"), (INSTR_Op (OP_IBinop (AShr false) (DTYPE_I 64%N) EXP_Undef EXP_Undef)))];
+      blk_term := TERM_Ret ((DTYPE_I 64%N), (EXP_Ident (ID_Local (Name "r"))));
       blk_comments := None
     |}.
 
@@ -175,8 +175,8 @@ Definition undef_test12b_block : block dtyp
   := {|
       blk_id := (Anon 0%Z);
       blk_phis := [];
-      blk_code := [(IId (Name "r"), (INSTR_Op (OP_IBinop (AShr false) (DTYPE_I 64%Z) (EXP_Ident (ID_Local (Name "a"))) EXP_Undef)))];
-      blk_term := (IVoid 0%Z, TERM_Ret ((DTYPE_I 64%Z), (EXP_Ident (ID_Local (Name "r")))));
+      blk_code := [(IId (Name "r"), (INSTR_Op (OP_IBinop (AShr false) (DTYPE_I 64%N) (EXP_Ident (ID_Local (Name "a"))) EXP_Undef)))];
+      blk_term := TERM_Ret ((DTYPE_I 64%N), (EXP_Ident (ID_Local (Name "r"))));
       blk_comments := None
     |}.
 
@@ -184,8 +184,8 @@ Definition undef_test13_block : block dtyp
   := {|
       blk_id := (Anon 0%Z);
       blk_phis := [];
-      blk_code := [(IId (Name "r"), (INSTR_Op (OP_IBinop (LShr false) (DTYPE_I 64%Z) EXP_Undef EXP_Undef)))];
-      blk_term := (IVoid 0%Z, TERM_Ret ((DTYPE_I 64%Z), (EXP_Ident (ID_Local (Name "r")))));
+      blk_code := [(IId (Name "r"), (INSTR_Op (OP_IBinop (LShr false) (DTYPE_I 64%N) EXP_Undef EXP_Undef)))];
+      blk_term := TERM_Ret ((DTYPE_I 64%N), (EXP_Ident (ID_Local (Name "r"))));
       blk_comments := None
     |}.
 
@@ -193,8 +193,8 @@ Definition undef_test13b_block : block dtyp
   := {|
       blk_id := (Anon 0%Z);
       blk_phis := [];
-      blk_code := [(IId (Name "r"), (INSTR_Op (OP_IBinop (LShr false) (DTYPE_I 64%Z) (EXP_Ident (ID_Local (Name "a"))) EXP_Undef)))];
-      blk_term := (IVoid 0%Z, TERM_Ret ((DTYPE_I 64%Z), (EXP_Ident (ID_Local (Name "r")))));
+      blk_code := [(IId (Name "r"), (INSTR_Op (OP_IBinop (LShr false) (DTYPE_I 64%N) (EXP_Ident (ID_Local (Name "a"))) EXP_Undef)))];
+      blk_term := TERM_Ret ((DTYPE_I 64%N), (EXP_Ident (ID_Local (Name "r"))));
       blk_comments := None
     |}.
 
@@ -202,8 +202,8 @@ Definition undef_test14_block : block dtyp
   := {|
       blk_id := (Anon 0%Z);
       blk_phis := [];
-      blk_code := [(IId (Name "r"), (INSTR_Op (OP_ICmp Slt (DTYPE_I 64%Z) EXP_Undef EXP_Undef)))];
-      blk_term := (IVoid 0%Z, TERM_Ret ((DTYPE_I 1%Z), (EXP_Ident (ID_Local (Name "r")))));
+      blk_code := [(IId (Name "r"), (INSTR_Op (OP_ICmp Slt (DTYPE_I 64%N) EXP_Undef EXP_Undef)))];
+      blk_term := TERM_Ret ((DTYPE_I 1%N), (EXP_Ident (ID_Local (Name "r"))));
       blk_comments := None
     |}.
 
@@ -211,8 +211,8 @@ Definition undef_test15_block : block dtyp
   := {|
       blk_id := (Anon 0%Z);
       blk_phis := [];
-      blk_code := [(IId (Name "r"), (INSTR_Op (OP_ICmp Ult (DTYPE_I 64%Z) EXP_Undef EXP_Undef)))];
-      blk_term := (IVoid 0%Z, TERM_Ret ((DTYPE_I 1%Z), (EXP_Ident (ID_Local (Name "r")))));
+      blk_code := [(IId (Name "r"), (INSTR_Op (OP_ICmp Ult (DTYPE_I 64%N) EXP_Undef EXP_Undef)))];
+      blk_term := TERM_Ret ((DTYPE_I 1%N), (EXP_Ident (ID_Local (Name "r"))));
       blk_comments := None
     |}.
 
@@ -220,8 +220,8 @@ Definition undef_test16_block : block dtyp
   := {|
       blk_id := (Anon 0%Z);
       blk_phis := [];
-      blk_code := [(IId (Name "r"), (INSTR_Op (OP_Select ((DTYPE_I 1%Z),EXP_Undef) ((DTYPE_I 64%Z),(EXP_Ident (ID_Local (Name "a")))) ((DTYPE_I 64%Z),EXP_Undef))))];
-      blk_term := (IVoid 0%Z, TERM_Ret ((DTYPE_I 64%Z), (EXP_Ident (ID_Local (Name "r")))));
+      blk_code := [(IId (Name "r"), (INSTR_Op (OP_Select ((DTYPE_I 1%N),EXP_Undef) ((DTYPE_I 64%N),(EXP_Ident (ID_Local (Name "a")))) ((DTYPE_I 64%N),EXP_Undef))))];
+      blk_term := TERM_Ret ((DTYPE_I 64%N), (EXP_Ident (ID_Local (Name "r"))));
       blk_comments := None
     |}.
 
@@ -229,8 +229,8 @@ Definition undef_test17_block : block dtyp
   := {|
       blk_id := (Anon 0%Z);
       blk_phis := [];
-      blk_code := [(IId (Name "r"), (INSTR_Op (OP_Select ((DTYPE_I 1%Z),EXP_Undef) ((DTYPE_I 64%Z),EXP_Undef) ((DTYPE_I 64%Z),(EXP_Ident (ID_Local (Name "a")))))))];
-      blk_term := (IVoid 0%Z, TERM_Ret ((DTYPE_I 64%Z), (EXP_Ident (ID_Local (Name "r")))));
+      blk_code := [(IId (Name "r"), (INSTR_Op (OP_Select ((DTYPE_I 1%N),EXP_Undef) ((DTYPE_I 64%N),EXP_Undef) ((DTYPE_I 64%N),(EXP_Ident (ID_Local (Name "a")))))))];
+      blk_term := TERM_Ret ((DTYPE_I 64%N), (EXP_Ident (ID_Local (Name "r"))));
       blk_comments := None
     |}.
 
@@ -238,8 +238,8 @@ Definition undef_test18_block : block dtyp
   := {|
       blk_id := (Anon 0%Z);
       blk_phis := [];
-      blk_code := [(IId (Name "r"), (INSTR_Call ((DTYPE_Pointer), @EXP_Undef dtyp) [((DTYPE_I 64%Z), (EXP_Ident (ID_Local (Name "a"))))]))];
-      blk_term := (IVoid 0%Z, TERM_Ret ((DTYPE_I 64%Z), (EXP_Ident (ID_Local (Name "r")))));
+      blk_code := [(IId (Name "r"), (INSTR_Call ((DTYPE_Pointer), @EXP_Undef dtyp) [((DTYPE_I 64%N), (EXP_Ident (ID_Local (Name "a"))))]))];
+      blk_term := TERM_Ret ((DTYPE_I 64%N), (EXP_Ident (ID_Local (Name "r"))));
       blk_comments := None
     |}.
 
@@ -247,8 +247,8 @@ Definition undef_test19_block : block dtyp
   := {|
       blk_id := (Anon 0%Z);
       blk_phis := [];
-      blk_code := [(IId (Name "b"), (INSTR_Op (OP_IBinop (Shl false false) (DTYPE_Vector 4%Z (DTYPE_I 8%Z)) (EXP_Ident (ID_Local (Name "a"))) (EXP_Vector [((DTYPE_I 8%Z),(EXP_Integer 8%Z)); ((DTYPE_I 8%Z),(EXP_Integer 9%Z)); ((DTYPE_I 8%Z),EXP_Undef); ((DTYPE_I 8%Z), (EXP_Integer (-1)%Z))]))))];
-      blk_term := (IVoid 0%Z, TERM_Ret ((DTYPE_Vector 4%Z (DTYPE_I 8%Z)), (EXP_Ident (ID_Local (Name "b")))));
+      blk_code := [(IId (Name "b"), (INSTR_Op (OP_IBinop (Shl false false) (DTYPE_Vector 4%N (DTYPE_I 8%N)) (EXP_Ident (ID_Local (Name "a"))) (EXP_Vector [((DTYPE_I 8%N),(EXP_Integer 8%Z)); ((DTYPE_I 8%N),(EXP_Integer 9%Z)); ((DTYPE_I 8%N),EXP_Undef); ((DTYPE_I 8%N), (EXP_Integer (-1)%Z))]))))];
+      blk_term := TERM_Ret ((DTYPE_Vector 4%N (DTYPE_I 8%N)), (EXP_Ident (ID_Local (Name "b"))));
       blk_comments := None
     |}.
 
@@ -256,8 +256,8 @@ Definition undef_test20_block : block dtyp
   := {|
       blk_id := (Anon 0%Z);
       blk_phis := [];
-      blk_code := [(IId (Name "b"), (INSTR_Op (OP_IBinop (UDiv false) (DTYPE_I 32%Z) (EXP_Ident (ID_Local (Name "a"))) (EXP_Integer 0%Z))))];
-      blk_term := (IVoid 0%Z, TERM_Ret ((DTYPE_I 32%Z), (EXP_Ident (ID_Local (Name "b")))));
+      blk_code := [(IId (Name "b"), (INSTR_Op (OP_IBinop (UDiv false) (DTYPE_I 32%N) (EXP_Ident (ID_Local (Name "a"))) (EXP_Integer 0%Z))))];
+      blk_term := TERM_Ret ((DTYPE_I 32%N), (EXP_Ident (ID_Local (Name "b"))));
       blk_comments := None
     |}.
 
@@ -265,8 +265,8 @@ Definition undef_test20vec_block : block dtyp
   := {|
       blk_id := (Anon 0%Z);
       blk_phis := [];
-      blk_code := [(IId (Name "b"), (INSTR_Op (OP_IBinop (UDiv false) (DTYPE_Vector 2%Z (DTYPE_I 32%Z)) (EXP_Ident (ID_Local (Name "a"))) EXP_Zero_initializer)))];
-      blk_term := (IVoid 0%Z, TERM_Ret ((DTYPE_Vector 2%Z (DTYPE_I 32%Z)), (EXP_Ident (ID_Local (Name "b")))));
+      blk_code := [(IId (Name "b"), (INSTR_Op (OP_IBinop (UDiv false) (DTYPE_Vector 2%N (DTYPE_I 32%N)) (EXP_Ident (ID_Local (Name "a"))) EXP_Zero_initializer)))];
+      blk_term := TERM_Ret ((DTYPE_Vector 2%N (DTYPE_I 32%N)), (EXP_Ident (ID_Local (Name "b"))));
       blk_comments := None
     |}.
 
@@ -274,8 +274,8 @@ Definition undef_test21_block : block dtyp
   := {|
       blk_id := (Anon 0%Z);
       blk_phis := [];
-      blk_code := [(IId (Name "b"), (INSTR_Op (OP_IBinop (SDiv false) (DTYPE_I 32%Z) (EXP_Ident (ID_Local (Name "a"))) (EXP_Integer 0%Z))))];
-      blk_term := (IVoid 0%Z, TERM_Ret ((DTYPE_I 32%Z), (EXP_Ident (ID_Local (Name "b")))));
+      blk_code := [(IId (Name "b"), (INSTR_Op (OP_IBinop (SDiv false) (DTYPE_I 32%N) (EXP_Ident (ID_Local (Name "a"))) (EXP_Integer 0%Z))))];
+      blk_term := TERM_Ret ((DTYPE_I 32%N), (EXP_Ident (ID_Local (Name "b"))));
       blk_comments := None
     |}.
 
@@ -283,8 +283,8 @@ Definition undef_test21vec_block : block dtyp
   := {|
       blk_id := (Anon 0%Z);
       blk_phis := [];
-      blk_code := [(IId (Name "b"), (INSTR_Op (OP_IBinop (SDiv false) (DTYPE_Vector 2%Z (DTYPE_I 32%Z)) (EXP_Ident (ID_Local (Name "a"))) EXP_Zero_initializer)))];
-      blk_term := (IVoid 0%Z, TERM_Ret ((DTYPE_Vector 2%Z (DTYPE_I 32%Z)), (EXP_Ident (ID_Local (Name "b")))));
+      blk_code := [(IId (Name "b"), (INSTR_Op (OP_IBinop (SDiv false) (DTYPE_Vector 2%N (DTYPE_I 32%N)) (EXP_Ident (ID_Local (Name "a"))) EXP_Zero_initializer)))];
+      blk_term := TERM_Ret ((DTYPE_Vector 2%N (DTYPE_I 32%N)), (EXP_Ident (ID_Local (Name "b"))));
       blk_comments := None
     |}.
 
@@ -292,8 +292,8 @@ Definition undef_test22_block : block dtyp
   := {|
       blk_id := (Anon 0%Z);
       blk_phis := [];
-      blk_code := [(IId (Name "b"), (INSTR_Op (OP_IBinop (AShr true) (DTYPE_I 32%Z) EXP_Undef (EXP_Ident (ID_Local (Name "a"))))))];
-      blk_term := (IVoid 0%Z, TERM_Ret ((DTYPE_I 32%Z), (EXP_Ident (ID_Local (Name "b")))));
+      blk_code := [(IId (Name "b"), (INSTR_Op (OP_IBinop (AShr true) (DTYPE_I 32%N) EXP_Undef (EXP_Ident (ID_Local (Name "a"))))))];
+      blk_term := TERM_Ret ((DTYPE_I 32%N), (EXP_Ident (ID_Local (Name "b"))));
       blk_comments := None
     |}.
 
@@ -301,8 +301,8 @@ Definition undef_test23_block : block dtyp
   := {|
       blk_id := (Anon 0%Z);
       blk_phis := [];
-      blk_code := [(IId (Name "b"), (INSTR_Op (OP_IBinop (LShr true) (DTYPE_I 32%Z) EXP_Undef (EXP_Ident (ID_Local (Name "a"))))))];
-      blk_term := (IVoid 0%Z, TERM_Ret ((DTYPE_I 32%Z), (EXP_Ident (ID_Local (Name "b")))));
+      blk_code := [(IId (Name "b"), (INSTR_Op (OP_IBinop (LShr true) (DTYPE_I 32%N) EXP_Undef (EXP_Ident (ID_Local (Name "a"))))))];
+      blk_term := TERM_Ret ((DTYPE_I 32%N), (EXP_Ident (ID_Local (Name "b"))));
       blk_comments := None
     |}.
 
@@ -310,8 +310,8 @@ Definition undef_test24_block : block dtyp
   := {|
       blk_id := (Anon 0%Z);
       blk_phis := [];
-      blk_code := [(IId (Name "b"), (INSTR_Op (OP_IBinop (UDiv false) (DTYPE_I 32%Z) EXP_Undef (EXP_Integer 0%Z))))];
-      blk_term := (IVoid 0%Z, TERM_Ret ((DTYPE_I 32%Z), (EXP_Ident (ID_Local (Name "b")))));
+      blk_code := [(IId (Name "b"), (INSTR_Op (OP_IBinop (UDiv false) (DTYPE_I 32%N) EXP_Undef (EXP_Integer 0%Z))))];
+      blk_term := TERM_Ret ((DTYPE_I 32%N), (EXP_Ident (ID_Local (Name "b"))));
       blk_comments := None
     |}.
 
@@ -319,8 +319,8 @@ Definition undef_test25_block : block dtyp
   := {|
       blk_id := (Anon 0%Z);
       blk_phis := [];
-      blk_code := [(IId (Name "b"), (INSTR_Op (OP_IBinop (LShr false) (DTYPE_I 32%Z) (EXP_Integer 0%Z) EXP_Undef)))];
-      blk_term := (IVoid 0%Z, TERM_Ret ((DTYPE_I 32%Z), (EXP_Ident (ID_Local (Name "b")))));
+      blk_code := [(IId (Name "b"), (INSTR_Op (OP_IBinop (LShr false) (DTYPE_I 32%N) (EXP_Integer 0%Z) EXP_Undef)))];
+      blk_term := TERM_Ret ((DTYPE_I 32%N), (EXP_Ident (ID_Local (Name "b"))));
       blk_comments := None
     |}.
 
@@ -328,8 +328,8 @@ Definition undef_test26_block : block dtyp
   := {|
       blk_id := (Anon 0%Z);
       blk_phis := [];
-      blk_code := [(IId (Name "b"), (INSTR_Op (OP_IBinop (AShr false) (DTYPE_I 32%Z) (EXP_Integer 0%Z) EXP_Undef)))];
-      blk_term := (IVoid 0%Z, TERM_Ret ((DTYPE_I 32%Z), (EXP_Ident (ID_Local (Name "b")))));
+      blk_code := [(IId (Name "b"), (INSTR_Op (OP_IBinop (AShr false) (DTYPE_I 32%N) (EXP_Integer 0%Z) EXP_Undef)))];
+      blk_term := TERM_Ret ((DTYPE_I 32%N), (EXP_Ident (ID_Local (Name "b"))));
       blk_comments := None
     |}.
 
@@ -337,8 +337,8 @@ Definition undef_test27_block : block dtyp
   := {|
       blk_id := (Anon 0%Z);
       blk_phis := [];
-      blk_code := [(IId (Name "b"), (INSTR_Op (OP_IBinop (Shl false false) (DTYPE_I 32%Z) (EXP_Integer 0%Z) EXP_Undef)))];
-      blk_term := (IVoid 0%Z, TERM_Ret ((DTYPE_I 32%Z), (EXP_Ident (ID_Local (Name "b")))));
+      blk_code := [(IId (Name "b"), (INSTR_Op (OP_IBinop (Shl false false) (DTYPE_I 32%N) (EXP_Integer 0%Z) EXP_Undef)))];
+      blk_term := TERM_Ret ((DTYPE_I 32%N), (EXP_Ident (ID_Local (Name "b"))));
       blk_comments := None
     |}.
 
@@ -346,8 +346,8 @@ Definition undef_test28_block : block dtyp
   := {|
       blk_id := (Anon 0%Z);
       blk_phis := [];
-      blk_code := [(IId (Name "b"), (INSTR_Op (OP_IBinop (Shl false true) (DTYPE_I 32%Z) EXP_Undef (EXP_Ident (ID_Local (Name "a"))))))];
-      blk_term := (IVoid 0%Z, TERM_Ret ((DTYPE_I 32%Z), (EXP_Ident (ID_Local (Name "b")))));
+      blk_code := [(IId (Name "b"), (INSTR_Op (OP_IBinop (Shl false true) (DTYPE_I 32%N) EXP_Undef (EXP_Ident (ID_Local (Name "a"))))))];
+      blk_term := TERM_Ret ((DTYPE_I 32%N), (EXP_Ident (ID_Local (Name "b"))));
       blk_comments := None
     |}.
 
@@ -355,8 +355,8 @@ Definition undef_test29_block : block dtyp
   := {|
       blk_id := (Anon 0%Z);
       blk_phis := [];
-      blk_code := [(IId (Name "b"), (INSTR_Op (OP_IBinop (Shl true false) (DTYPE_I 32%Z) EXP_Undef (EXP_Ident (ID_Local (Name "a"))))))];
-      blk_term := (IVoid 0%Z, TERM_Ret ((DTYPE_I 32%Z), (EXP_Ident (ID_Local (Name "b")))));
+      blk_code := [(IId (Name "b"), (INSTR_Op (OP_IBinop (Shl true false) (DTYPE_I 32%N) EXP_Undef (EXP_Ident (ID_Local (Name "a"))))))];
+      blk_term := TERM_Ret ((DTYPE_I 32%N), (EXP_Ident (ID_Local (Name "b"))));
       blk_comments := None
     |}.
 
@@ -364,8 +364,8 @@ Definition undef_test30_block : block dtyp
   := {|
       blk_id := (Anon 0%Z);
       blk_phis := [];
-      blk_code := [(IId (Name "b"), (INSTR_Op (OP_IBinop (Shl true true) (DTYPE_I 32%Z) EXP_Undef (EXP_Ident (ID_Local (Name "a"))))))];
-      blk_term := (IVoid 0%Z, TERM_Ret ((DTYPE_I 32%Z), (EXP_Ident (ID_Local (Name "b")))));
+      blk_code := [(IId (Name "b"), (INSTR_Op (OP_IBinop (Shl true true) (DTYPE_I 32%N) EXP_Undef (EXP_Ident (ID_Local (Name "a"))))))];
+      blk_term := TERM_Ret ((DTYPE_I 32%N), (EXP_Ident (ID_Local (Name "b"))));
       blk_comments := None
     |}.
 
@@ -373,8 +373,8 @@ Definition undef_test31_block : block dtyp
   := {|
       blk_id := (Anon 0%Z);
       blk_phis := [];
-      blk_code := [(IId (Name "b"), (INSTR_Op (OP_IBinop (Shl false false) (DTYPE_I 32%Z) EXP_Undef (EXP_Ident (ID_Local (Name "a"))))))];
-      blk_term := (IVoid 0%Z, TERM_Ret ((DTYPE_I 32%Z), (EXP_Ident (ID_Local (Name "b")))));
+      blk_code := [(IId (Name "b"), (INSTR_Op (OP_IBinop (Shl false false) (DTYPE_I 32%N) EXP_Undef (EXP_Ident (ID_Local (Name "a"))))))];
+      blk_term := TERM_Ret ((DTYPE_I 32%N), (EXP_Ident (ID_Local (Name "b"))));
       blk_comments := None
     |}.
 
@@ -382,8 +382,8 @@ Definition undef_test32_block : block dtyp
   := {|
       blk_id := (Anon 0%Z);
       blk_phis := [];
-      blk_code := [(IId (Name "b"), (INSTR_Op (OP_IBinop (Shl false false) (DTYPE_I 32%Z) EXP_Undef (EXP_Integer 0%Z))))];
-      blk_term := (IVoid 0%Z, TERM_Ret ((DTYPE_I 32%Z), (EXP_Ident (ID_Local (Name "b")))));
+      blk_code := [(IId (Name "b"), (INSTR_Op (OP_IBinop (Shl false false) (DTYPE_I 32%N) EXP_Undef (EXP_Integer 0%Z))))];
+      blk_term := TERM_Ret ((DTYPE_I 32%N), (EXP_Ident (ID_Local (Name "b"))));
       blk_comments := None
     |}.
 
@@ -391,8 +391,8 @@ Definition undef_test33_block : block dtyp
   := {|
       blk_id := (Anon 0%Z);
       blk_phis := [];
-      blk_code := [(IId (Name "b"), (INSTR_Op (OP_IBinop (AShr false) (DTYPE_I 32%Z) EXP_Undef (EXP_Integer 0%Z))))];
-      blk_term := (IVoid 0%Z, TERM_Ret ((DTYPE_I 32%Z), (EXP_Ident (ID_Local (Name "b")))));
+      blk_code := [(IId (Name "b"), (INSTR_Op (OP_IBinop (AShr false) (DTYPE_I 32%N) EXP_Undef (EXP_Integer 0%Z))))];
+      blk_term := TERM_Ret ((DTYPE_I 32%N), (EXP_Ident (ID_Local (Name "b"))));
       blk_comments := None
     |}.
 
@@ -400,8 +400,8 @@ Definition undef_test34_block : block dtyp
   := {|
       blk_id := (Anon 0%Z);
       blk_phis := [];
-      blk_code := [(IId (Name "b"), (INSTR_Op (OP_IBinop (LShr false) (DTYPE_I 32%Z) EXP_Undef (EXP_Integer 0%Z))))];
-      blk_term := (IVoid 0%Z, TERM_Ret ((DTYPE_I 32%Z), (EXP_Ident (ID_Local (Name "b")))));
+      blk_code := [(IId (Name "b"), (INSTR_Op (OP_IBinop (LShr false) (DTYPE_I 32%N) EXP_Undef (EXP_Integer 0%Z))))];
+      blk_term := TERM_Ret ((DTYPE_I 32%N), (EXP_Ident (ID_Local (Name "b"))));
       blk_comments := None
     |}.
 
@@ -409,8 +409,8 @@ Definition undef_test35_block : block dtyp
   := {|
       blk_id := (Anon 0%Z);
       blk_phis := [];
-      blk_code := [(IId (Name "b"), (INSTR_Op (OP_ExtractElement ((DTYPE_Vector 4%Z (DTYPE_I 32%Z)),(EXP_Ident (ID_Local (Name "V")))) ((DTYPE_I 32%Z),(EXP_Integer 4%Z)))))];
-      blk_term := (IVoid 0%Z, TERM_Ret ((DTYPE_I 32%Z), (EXP_Ident (ID_Local (Name "b")))));
+      blk_code := [(IId (Name "b"), (INSTR_Op (OP_ExtractElement ((DTYPE_Vector 4%N (DTYPE_I 32%N)),(EXP_Ident (ID_Local (Name "V")))) ((DTYPE_I 32%N),(EXP_Integer 4%Z)))))];
+      blk_term := TERM_Ret ((DTYPE_I 32%N), (EXP_Ident (ID_Local (Name "b"))));
       blk_comments := None
     |}.
 
@@ -418,8 +418,8 @@ Definition undef_test36_block : block dtyp
   := {|
       blk_id := (Anon 0%Z);
       blk_phis := [];
-      blk_code := [(IId (Name "b"), (INSTR_Op (OP_ExtractElement ((DTYPE_Vector 4%Z (DTYPE_I 32%Z)),EXP_Undef) ((DTYPE_I 32%Z),(EXP_Ident (ID_Local (Name "V")))))))];
-      blk_term := (IVoid 0%Z, TERM_Ret ((DTYPE_I 32%Z), (EXP_Ident (ID_Local (Name "b")))));
+      blk_code := [(IId (Name "b"), (INSTR_Op (OP_ExtractElement ((DTYPE_Vector 4%N (DTYPE_I 32%N)),EXP_Undef) ((DTYPE_I 32%N),(EXP_Ident (ID_Local (Name "V")))))))];
+      blk_term := TERM_Ret ((DTYPE_I 32%N), (EXP_Ident (ID_Local (Name "b"))));
       blk_comments := None
     |}.
 
@@ -427,8 +427,8 @@ Definition undef_test37_block : block dtyp
   := {|
       blk_id := (Anon 0%Z);
       blk_phis := [];
-      blk_code := [(IId (Name "b"), (INSTR_Op (OP_IBinop (UDiv false) (DTYPE_I 32%Z) EXP_Undef EXP_Undef)))];
-      blk_term := (IVoid 0%Z, TERM_Ret ((DTYPE_I 32%Z), (EXP_Ident (ID_Local (Name "b")))));
+      blk_code := [(IId (Name "b"), (INSTR_Op (OP_IBinop (UDiv false) (DTYPE_I 32%N) EXP_Undef EXP_Undef)))];
+      blk_term := TERM_Ret ((DTYPE_I 32%N), (EXP_Ident (ID_Local (Name "b"))));
       blk_comments := None
     |}.
 
@@ -436,8 +436,8 @@ Definition undef_test38_block : block dtyp
   := {|
       blk_id := (Anon 0%Z);
       blk_phis := [];
-      blk_code := [(IId (Name "b"), (INSTR_Op (OP_IBinop (UDiv false) (DTYPE_I 32%Z) (EXP_Ident (ID_Local (Name "a"))) EXP_Undef)))];
-      blk_term := (IVoid 0%Z, TERM_Ret ((DTYPE_I 32%Z), (EXP_Ident (ID_Local (Name "b")))));
+      blk_code := [(IId (Name "b"), (INSTR_Op (OP_IBinop (UDiv false) (DTYPE_I 32%N) (EXP_Ident (ID_Local (Name "a"))) EXP_Undef)))];
+      blk_term := TERM_Ret ((DTYPE_I 32%N), (EXP_Ident (ID_Local (Name "b"))));
       blk_comments := None
     |}.
 
@@ -445,8 +445,8 @@ Definition undef_test39_block : block dtyp
   := {|
       blk_id := (Anon 0%Z);
       blk_phis := [];
-      blk_code := [(IId (Name "b"), (INSTR_Op (OP_IBinop (UDiv false) (DTYPE_I 32%Z) (EXP_Integer 0%Z) EXP_Undef)))];
-      blk_term := (IVoid 0%Z, TERM_Ret ((DTYPE_I 32%Z), (EXP_Ident (ID_Local (Name "b")))));
+      blk_code := [(IId (Name "b"), (INSTR_Op (OP_IBinop (UDiv false) (DTYPE_I 32%N) (EXP_Integer 0%Z) EXP_Undef)))];
+      blk_term := TERM_Ret ((DTYPE_I 32%N), (EXP_Ident (ID_Local (Name "b"))));
       blk_comments := None
     |}.
 
@@ -457,8 +457,8 @@ Definition undef_test0_cfg : cfg dtyp :=
      blks := [{|
                  blk_id := (Anon 0%Z);
                  blk_phis := [];
-                 blk_code := [(IId (Name "r"), (INSTR_Op (OP_IBinop (Mul false false) (DTYPE_I 64%Z) EXP_Undef EXP_Undef)))];
-                 blk_term := (IVoid 0%Z, TERM_Ret ((DTYPE_I 64%Z), (EXP_Ident (ID_Local (Name "r")))));
+                 blk_code := [(IId (Name "r"), (INSTR_Op (OP_IBinop (Mul false false) (DTYPE_I 64%N) EXP_Undef EXP_Undef)))];
+                 blk_term := TERM_Ret ((DTYPE_I 64%N), (EXP_Ident (ID_Local (Name "r"))));
                  blk_comments := None
                |}];
      args := [];
@@ -467,7 +467,7 @@ Definition undef_test0_cfg : cfg dtyp :=
 Definition undef_test0 : list (toplevel_entity typ (list (block typ)))
   := [TLE_Definition {|
           df_prototype := {|dc_name := (Name "main");
-                            dc_type := (TYPE_Function (TYPE_I 64%Z) []);
+                            dc_type := (TYPE_Function (TYPE_I 64%N) []);
                             dc_param_attrs := ([], []);
                             dc_linkage := None;
                             dc_visibility := None;
@@ -482,8 +482,8 @@ Definition undef_test0 : list (toplevel_entity typ (list (block typ)))
                         {|
                           blk_id := (Anon 0%Z);
                           blk_phis := [];
-                          blk_code := [(IId (Name "r"), (INSTR_Op (OP_IBinop (Mul false false) (TYPE_I 64%Z) EXP_Undef EXP_Undef)))];
-                          blk_term := (IVoid 0%Z, TERM_Ret ((TYPE_I 64%Z), (EXP_Ident (ID_Local (Name "r")))));
+                          blk_code := [(IId (Name "r"), (INSTR_Op (OP_IBinop (Mul false false) (TYPE_I 64%N) EXP_Undef EXP_Undef)))];
+                          blk_term := TERM_Ret ((TYPE_I 64%N), (EXP_Ident (ID_Local (Name "r"))));
                           blk_comments := None
                         |}]
         |}].
@@ -491,7 +491,7 @@ Definition undef_test0 : list (toplevel_entity typ (list (block typ)))
 Definition undef_test0_refine : list (toplevel_entity typ (list (block typ)))
   := [TLE_Definition {|
           df_prototype := {|dc_name := (Name "main");
-                            dc_type := (TYPE_Function (TYPE_I 64%Z) []);
+                            dc_type := (TYPE_Function (TYPE_I 64%N) []);
                             dc_param_attrs := ([], []);
                             dc_linkage := None;
                             dc_visibility := None;
@@ -507,7 +507,7 @@ Definition undef_test0_refine : list (toplevel_entity typ (list (block typ)))
                           blk_id := (Anon 0%Z);
                           blk_phis := [];
                           blk_code := [];
-                          blk_term := (IVoid 0%Z, TERM_Ret ((TYPE_I 64%Z), (EXP_Undef)));
+                          blk_term := TERM_Ret ((TYPE_I 64%N), (EXP_Undef));
                           blk_comments := None
                         |}]
         |}].
@@ -516,7 +516,7 @@ Definition undef_test0_refine : list (toplevel_entity typ (list (block typ)))
 Definition undef_test1 : list (toplevel_entity typ (list (block typ)))
   := [TLE_Definition {|
           df_prototype := {|dc_name := (Name "test1");
-                            dc_type := (TYPE_Function (TYPE_I 64%Z) []);
+                            dc_type := (TYPE_Function (TYPE_I 64%N) []);
                             dc_param_attrs := ([], []);
                             dc_linkage := None;
                             dc_visibility := None;
@@ -531,8 +531,8 @@ Definition undef_test1 : list (toplevel_entity typ (list (block typ)))
                         {|
                           blk_id := (Anon 0%Z);
                           blk_phis := [];
-                          blk_code := [(IId (Name "r"), (INSTR_Op (OP_IBinop (Mul false false) (TYPE_I 64%Z) (EXP_Integer 3%Z) EXP_Undef)))];
-                          blk_term := (IVoid 0%Z, TERM_Ret ((TYPE_I 64%Z), (EXP_Ident (ID_Local (Name "r")))));
+                          blk_code := [(IId (Name "r"), (INSTR_Op (OP_IBinop (Mul false false) (TYPE_I 64%N) (EXP_Integer 3%Z) EXP_Undef)))];
+                          blk_term := TERM_Ret ((TYPE_I 64%N), (EXP_Ident (ID_Local (Name "r"))));
                           blk_comments := None
                         |}]
         |}].
@@ -540,7 +540,7 @@ Definition undef_test1 : list (toplevel_entity typ (list (block typ)))
 Definition undef_test2 : list (toplevel_entity typ (list (block typ)))
   := [TLE_Definition {|
           df_prototype := {|dc_name := (Name "test2");
-                            dc_type := (TYPE_Function (TYPE_I 64%Z) []);
+                            dc_type := (TYPE_Function (TYPE_I 64%N) []);
                             dc_param_attrs := ([], []);
                             dc_linkage := None;
                             dc_visibility := None;
@@ -555,8 +555,8 @@ Definition undef_test2 : list (toplevel_entity typ (list (block typ)))
                         {|
                           blk_id := (Anon 0%Z);
                           blk_phis := [];
-                          blk_code := [(IId (Name "r"), (INSTR_Op (OP_IBinop (Mul false false) (TYPE_I 64%Z) EXP_Undef (EXP_Integer 3%Z))))];
-                          blk_term := (IVoid 0%Z, TERM_Ret ((TYPE_I 64%Z), (EXP_Ident (ID_Local (Name "r")))));
+                          blk_code := [(IId (Name "r"), (INSTR_Op (OP_IBinop (Mul false false) (TYPE_I 64%N) EXP_Undef (EXP_Integer 3%Z))))];
+                          blk_term := TERM_Ret ((TYPE_I 64%N), (EXP_Ident (ID_Local (Name "r"))));
                           blk_comments := None
                         |}]
         |}].
@@ -564,7 +564,7 @@ Definition undef_test2 : list (toplevel_entity typ (list (block typ)))
 Definition undef_test3 : list (toplevel_entity typ (list (block typ)))
   := [TLE_Definition {|
           df_prototype := {|dc_name := (Name "test3");
-                            dc_type := (TYPE_Function (TYPE_I 64%Z) []);
+                            dc_type := (TYPE_Function (TYPE_I 64%N) []);
                             dc_param_attrs := ([], []);
                             dc_linkage := None;
                             dc_visibility := None;
@@ -579,8 +579,8 @@ Definition undef_test3 : list (toplevel_entity typ (list (block typ)))
                         {|
                           blk_id := (Anon 0%Z);
                           blk_phis := [];
-                          blk_code := [(IId (Name "r"), (INSTR_Op (OP_IBinop (Mul false false) (TYPE_I 64%Z) EXP_Undef (EXP_Integer 6%Z))))];
-                          blk_term := (IVoid 0%Z, TERM_Ret ((TYPE_I 64%Z), (EXP_Ident (ID_Local (Name "r")))));
+                          blk_code := [(IId (Name "r"), (INSTR_Op (OP_IBinop (Mul false false) (TYPE_I 64%N) EXP_Undef (EXP_Integer 6%Z))))];
+                          blk_term := TERM_Ret ((TYPE_I 64%N), (EXP_Ident (ID_Local (Name "r"))));
                           blk_comments := None
                         |}]
         |}].
@@ -588,7 +588,7 @@ Definition undef_test3 : list (toplevel_entity typ (list (block typ)))
 Definition undef_test4 : list (toplevel_entity typ (list (block typ)))
   := [TLE_Definition {|
           df_prototype := {|dc_name := (Name "test4");
-                            dc_type := (TYPE_Function (TYPE_I 64%Z) []);
+                            dc_type := (TYPE_Function (TYPE_I 64%N) []);
                             dc_param_attrs := ([], []);
                             dc_linkage := None;
                             dc_visibility := None;
@@ -603,8 +603,8 @@ Definition undef_test4 : list (toplevel_entity typ (list (block typ)))
                         {|
                           blk_id := (Anon 0%Z);
                           blk_phis := [];
-                          blk_code := [(IId (Name "r"), (INSTR_Op (OP_IBinop (Mul false false) (TYPE_I 64%Z) (EXP_Integer 6%Z) EXP_Undef)))];
-                          blk_term := (IVoid 0%Z, TERM_Ret ((TYPE_I 64%Z), (EXP_Ident (ID_Local (Name "r")))));
+                          blk_code := [(IId (Name "r"), (INSTR_Op (OP_IBinop (Mul false false) (TYPE_I 64%N) (EXP_Integer 6%Z) EXP_Undef)))];
+                          blk_term := TERM_Ret ((TYPE_I 64%N), (EXP_Ident (ID_Local (Name "r"))));
                           blk_comments := None
                         |}]
         |}].
@@ -612,7 +612,7 @@ Definition undef_test4 : list (toplevel_entity typ (list (block typ)))
 Definition undef_test5 : list (toplevel_entity typ (list (block typ)))
   := [TLE_Definition {|
           df_prototype := {|dc_name := (Name "test5");
-                            dc_type := (TYPE_Function (TYPE_I 64%Z) []);
+                            dc_type := (TYPE_Function (TYPE_I 64%N) []);
                             dc_param_attrs := ([], []);
                             dc_linkage := None;
                             dc_visibility := None;
@@ -627,8 +627,8 @@ Definition undef_test5 : list (toplevel_entity typ (list (block typ)))
                         {|
                           blk_id := (Anon 0%Z);
                           blk_phis := [];
-                          blk_code := [(IId (Name "r"), (INSTR_Op (OP_IBinop And (TYPE_I 64%Z) EXP_Undef EXP_Undef)))];
-                          blk_term := (IVoid 0%Z, TERM_Ret ((TYPE_I 64%Z), (EXP_Ident (ID_Local (Name "r")))));
+                          blk_code := [(IId (Name "r"), (INSTR_Op (OP_IBinop And (TYPE_I 64%N) EXP_Undef EXP_Undef)))];
+                          blk_term := TERM_Ret ((TYPE_I 64%N), (EXP_Ident (ID_Local (Name "r"))));
                           blk_comments := None
                         |}]
         |}].
@@ -636,7 +636,7 @@ Definition undef_test5 : list (toplevel_entity typ (list (block typ)))
 Definition undef_test6 : list (toplevel_entity typ (list (block typ)))
   := [TLE_Definition {|
           df_prototype := {|dc_name := (Name "test6");
-                            dc_type := (TYPE_Function (TYPE_I 64%Z) []);
+                            dc_type := (TYPE_Function (TYPE_I 64%N) []);
                             dc_param_attrs := ([], []);
                             dc_linkage := None;
                             dc_visibility := None;
@@ -651,8 +651,8 @@ Definition undef_test6 : list (toplevel_entity typ (list (block typ)))
                         {|
                           blk_id := (Anon 0%Z);
                           blk_phis := [];
-                          blk_code := [(IId (Name "r"), (INSTR_Op (OP_IBinop Or (TYPE_I 64%Z) EXP_Undef EXP_Undef)))];
-                          blk_term := (IVoid 0%Z, TERM_Ret ((TYPE_I 64%Z), (EXP_Ident (ID_Local (Name "r")))));
+                          blk_code := [(IId (Name "r"), (INSTR_Op (OP_IBinop Or (TYPE_I 64%N) EXP_Undef EXP_Undef)))];
+                          blk_term := TERM_Ret ((TYPE_I 64%N), (EXP_Ident (ID_Local (Name "r"))));
                           blk_comments := None
                         |}]
         |}].
@@ -660,7 +660,7 @@ Definition undef_test6 : list (toplevel_entity typ (list (block typ)))
 Definition undef_test7 : list (toplevel_entity typ (list (block typ)))
   := [TLE_Definition {|
           df_prototype := {|dc_name := (Name "test7");
-                            dc_type := (TYPE_Function (TYPE_I 64%Z) []);
+                            dc_type := (TYPE_Function (TYPE_I 64%N) []);
                             dc_param_attrs := ([], []);
                             dc_linkage := None;
                             dc_visibility := None;
@@ -675,8 +675,8 @@ Definition undef_test7 : list (toplevel_entity typ (list (block typ)))
                         {|
                           blk_id := (Anon 0%Z);
                           blk_phis := [];
-                          blk_code := [(IId (Name "r"), (INSTR_Op (OP_IBinop (UDiv false) (TYPE_I 64%Z) EXP_Undef (EXP_Integer 1%Z))))];
-                          blk_term := (IVoid 0%Z, TERM_Ret ((TYPE_I 64%Z), (EXP_Ident (ID_Local (Name "r")))));
+                          blk_code := [(IId (Name "r"), (INSTR_Op (OP_IBinop (UDiv false) (TYPE_I 64%N) EXP_Undef (EXP_Integer 1%Z))))];
+                          blk_term := TERM_Ret ((TYPE_I 64%N), (EXP_Ident (ID_Local (Name "r"))));
                           blk_comments := None
                         |}]
         |}].
@@ -684,7 +684,7 @@ Definition undef_test7 : list (toplevel_entity typ (list (block typ)))
 Definition undef_test8 : list (toplevel_entity typ (list (block typ)))
   := [TLE_Definition {|
           df_prototype := {|dc_name := (Name "test8");
-                            dc_type := (TYPE_Function (TYPE_I 64%Z) []);
+                            dc_type := (TYPE_Function (TYPE_I 64%N) []);
                             dc_param_attrs := ([], []);
                             dc_linkage := None;
                             dc_visibility := None;
@@ -699,8 +699,8 @@ Definition undef_test8 : list (toplevel_entity typ (list (block typ)))
                         {|
                           blk_id := (Anon 0%Z);
                           blk_phis := [];
-                          blk_code := [(IId (Name "r"), (INSTR_Op (OP_IBinop (SDiv false) (TYPE_I 64%Z) EXP_Undef (EXP_Integer 1%Z))))];
-                          blk_term := (IVoid 0%Z, TERM_Ret ((TYPE_I 64%Z), (EXP_Ident (ID_Local (Name "r")))));
+                          blk_code := [(IId (Name "r"), (INSTR_Op (OP_IBinop (SDiv false) (TYPE_I 64%N) EXP_Undef (EXP_Integer 1%Z))))];
+                          blk_term := TERM_Ret ((TYPE_I 64%N), (EXP_Ident (ID_Local (Name "r"))));
                           blk_comments := None
                         |}]
         |}].
@@ -708,7 +708,7 @@ Definition undef_test8 : list (toplevel_entity typ (list (block typ)))
 Definition undef_test9 : list (toplevel_entity typ (list (block typ)))
   := [TLE_Definition {|
           df_prototype := {|dc_name := (Name "test9");
-                            dc_type := (TYPE_Function (TYPE_I 64%Z) []);
+                            dc_type := (TYPE_Function (TYPE_I 64%N) []);
                             dc_param_attrs := ([], []);
                             dc_linkage := None;
                             dc_visibility := None;
@@ -723,8 +723,8 @@ Definition undef_test9 : list (toplevel_entity typ (list (block typ)))
                         {|
                           blk_id := (Anon 0%Z);
                           blk_phis := [];
-                          blk_code := [(IId (Name "r"), (INSTR_Op (OP_IBinop URem (TYPE_I 64%Z) EXP_Undef (EXP_Integer 1%Z))))];
-                          blk_term := (IVoid 0%Z, TERM_Ret ((TYPE_I 64%Z), (EXP_Ident (ID_Local (Name "r")))));
+                          blk_code := [(IId (Name "r"), (INSTR_Op (OP_IBinop URem (TYPE_I 64%N) EXP_Undef (EXP_Integer 1%Z))))];
+                          blk_term := TERM_Ret ((TYPE_I 64%N), (EXP_Ident (ID_Local (Name "r"))));
                           blk_comments := None
                         |}]
         |}].
@@ -732,7 +732,7 @@ Definition undef_test9 : list (toplevel_entity typ (list (block typ)))
 Definition undef_test10 : list (toplevel_entity typ (list (block typ)))
   := [TLE_Definition {|
           df_prototype := {|dc_name := (Name "test10");
-                            dc_type := (TYPE_Function (TYPE_I 64%Z) []);
+                            dc_type := (TYPE_Function (TYPE_I 64%N) []);
                             dc_param_attrs := ([], []);
                             dc_linkage := None;
                             dc_visibility := None;
@@ -747,8 +747,8 @@ Definition undef_test10 : list (toplevel_entity typ (list (block typ)))
                         {|
                           blk_id := (Anon 0%Z);
                           blk_phis := [];
-                          blk_code := [(IId (Name "r"), (INSTR_Op (OP_IBinop SRem (TYPE_I 64%Z) EXP_Undef (EXP_Integer 1%Z))))];
-                          blk_term := (IVoid 0%Z, TERM_Ret ((TYPE_I 64%Z), (EXP_Ident (ID_Local (Name "r")))));
+                          blk_code := [(IId (Name "r"), (INSTR_Op (OP_IBinop SRem (TYPE_I 64%N) EXP_Undef (EXP_Integer 1%Z))))];
+                          blk_term := TERM_Ret ((TYPE_I 64%N), (EXP_Ident (ID_Local (Name "r"))));
                           blk_comments := None
                         |}]
         |}].
@@ -756,7 +756,7 @@ Definition undef_test10 : list (toplevel_entity typ (list (block typ)))
 Definition undef_test11 : list (toplevel_entity typ (list (block typ)))
   := [TLE_Definition {|
           df_prototype := {|dc_name := (Name "test11");
-                            dc_type := (TYPE_Function (TYPE_I 64%Z) []);
+                            dc_type := (TYPE_Function (TYPE_I 64%N) []);
                             dc_param_attrs := ([], []);
                             dc_linkage := None;
                             dc_visibility := None;
@@ -771,8 +771,8 @@ Definition undef_test11 : list (toplevel_entity typ (list (block typ)))
                         {|
                           blk_id := (Anon 0%Z);
                           blk_phis := [];
-                          blk_code := [(IId (Name "r"), (INSTR_Op (OP_IBinop (Shl false false) (TYPE_I 64%Z) EXP_Undef EXP_Undef)))];
-                          blk_term := (IVoid 0%Z, TERM_Ret ((TYPE_I 64%Z), (EXP_Ident (ID_Local (Name "r")))));
+                          blk_code := [(IId (Name "r"), (INSTR_Op (OP_IBinop (Shl false false) (TYPE_I 64%N) EXP_Undef EXP_Undef)))];
+                          blk_term := TERM_Ret ((TYPE_I 64%N), (EXP_Ident (ID_Local (Name "r"))));
                           blk_comments := None
                         |}]
         |}].
@@ -780,7 +780,7 @@ Definition undef_test11 : list (toplevel_entity typ (list (block typ)))
 Definition undef_test11b : list (toplevel_entity typ (list (block typ)))
   := [TLE_Definition {|
           df_prototype := {|dc_name := (Name "test11b");
-                            dc_type := (TYPE_Function (TYPE_I 64%Z) [(TYPE_I 64%Z)]);
+                            dc_type := (TYPE_Function (TYPE_I 64%N) [(TYPE_I 64%N)]);
                             dc_param_attrs := ([], []);
                             dc_linkage := None;
                             dc_visibility := None;
@@ -795,8 +795,8 @@ Definition undef_test11b : list (toplevel_entity typ (list (block typ)))
                         {|
                           blk_id := (Anon 0%Z);
                           blk_phis := [];
-                          blk_code := [(IId (Name "r"), (INSTR_Op (OP_IBinop (Shl false false) (TYPE_I 64%Z) (EXP_Ident (ID_Local (Name "a"))) EXP_Undef)))];
-                          blk_term := (IVoid 0%Z, TERM_Ret ((TYPE_I 64%Z), (EXP_Ident (ID_Local (Name "r")))));
+                          blk_code := [(IId (Name "r"), (INSTR_Op (OP_IBinop (Shl false false) (TYPE_I 64%N) (EXP_Ident (ID_Local (Name "a"))) EXP_Undef)))];
+                          blk_term := TERM_Ret ((TYPE_I 64%N), (EXP_Ident (ID_Local (Name "r"))));
                           blk_comments := None
                         |}]
         |}].
@@ -804,7 +804,7 @@ Definition undef_test11b : list (toplevel_entity typ (list (block typ)))
 Definition undef_test12 : list (toplevel_entity typ (list (block typ)))
   := [TLE_Definition {|
           df_prototype := {|dc_name := (Name "test12");
-                            dc_type := (TYPE_Function (TYPE_I 64%Z) []);
+                            dc_type := (TYPE_Function (TYPE_I 64%N) []);
                             dc_param_attrs := ([], []);
                             dc_linkage := None;
                             dc_visibility := None;
@@ -819,8 +819,8 @@ Definition undef_test12 : list (toplevel_entity typ (list (block typ)))
                         {|
                           blk_id := (Anon 0%Z);
                           blk_phis := [];
-                          blk_code := [(IId (Name "r"), (INSTR_Op (OP_IBinop (AShr false) (TYPE_I 64%Z) EXP_Undef EXP_Undef)))];
-                          blk_term := (IVoid 0%Z, TERM_Ret ((TYPE_I 64%Z), (EXP_Ident (ID_Local (Name "r")))));
+                          blk_code := [(IId (Name "r"), (INSTR_Op (OP_IBinop (AShr false) (TYPE_I 64%N) EXP_Undef EXP_Undef)))];
+                          blk_term := TERM_Ret ((TYPE_I 64%N), (EXP_Ident (ID_Local (Name "r"))));
                           blk_comments := None
                         |}]
         |}].
@@ -828,7 +828,7 @@ Definition undef_test12 : list (toplevel_entity typ (list (block typ)))
 Definition undef_test12b : list (toplevel_entity typ (list (block typ)))
   := [TLE_Definition {|
           df_prototype := {|dc_name := (Name "test12b");
-                            dc_type := (TYPE_Function (TYPE_I 64%Z) [(TYPE_I 64%Z)]);
+                            dc_type := (TYPE_Function (TYPE_I 64%N) [(TYPE_I 64%N)]);
                             dc_param_attrs := ([], []);
                             dc_linkage := None;
                             dc_visibility := None;
@@ -843,8 +843,8 @@ Definition undef_test12b : list (toplevel_entity typ (list (block typ)))
                         {|
                           blk_id := (Anon 0%Z);
                           blk_phis := [];
-                          blk_code := [(IId (Name "r"), (INSTR_Op (OP_IBinop (AShr false) (TYPE_I 64%Z) (EXP_Ident (ID_Local (Name "a"))) EXP_Undef)))];
-                          blk_term := (IVoid 0%Z, TERM_Ret ((TYPE_I 64%Z), (EXP_Ident (ID_Local (Name "r")))));
+                          blk_code := [(IId (Name "r"), (INSTR_Op (OP_IBinop (AShr false) (TYPE_I 64%N) (EXP_Ident (ID_Local (Name "a"))) EXP_Undef)))];
+                          blk_term := TERM_Ret ((TYPE_I 64%N), (EXP_Ident (ID_Local (Name "r"))));
                           blk_comments := None
                         |}]
         |}].
@@ -852,7 +852,7 @@ Definition undef_test12b : list (toplevel_entity typ (list (block typ)))
 Definition undef_test13 : list (toplevel_entity typ (list (block typ)))
   := [TLE_Definition {|
           df_prototype := {|dc_name := (Name "test13");
-                            dc_type := (TYPE_Function (TYPE_I 64%Z) []);
+                            dc_type := (TYPE_Function (TYPE_I 64%N) []);
                             dc_param_attrs := ([], []);
                             dc_linkage := None;
                             dc_visibility := None;
@@ -867,8 +867,8 @@ Definition undef_test13 : list (toplevel_entity typ (list (block typ)))
                         {|
                           blk_id := (Anon 0%Z);
                           blk_phis := [];
-                          blk_code := [(IId (Name "r"), (INSTR_Op (OP_IBinop (LShr false) (TYPE_I 64%Z) EXP_Undef EXP_Undef)))];
-                          blk_term := (IVoid 0%Z, TERM_Ret ((TYPE_I 64%Z), (EXP_Ident (ID_Local (Name "r")))));
+                          blk_code := [(IId (Name "r"), (INSTR_Op (OP_IBinop (LShr false) (TYPE_I 64%N) EXP_Undef EXP_Undef)))];
+                          blk_term := TERM_Ret ((TYPE_I 64%N), (EXP_Ident (ID_Local (Name "r"))));
                           blk_comments := None
                         |}]
         |}].
@@ -876,7 +876,7 @@ Definition undef_test13 : list (toplevel_entity typ (list (block typ)))
 Definition undef_test13b : list (toplevel_entity typ (list (block typ)))
   := [TLE_Definition {|
           df_prototype := {|dc_name := (Name "test13b");
-                            dc_type := (TYPE_Function (TYPE_I 64%Z) [(TYPE_I 64%Z)]);
+                            dc_type := (TYPE_Function (TYPE_I 64%N) [(TYPE_I 64%N)]);
                             dc_param_attrs := ([], []);
                             dc_linkage := None;
                             dc_visibility := None;
@@ -891,8 +891,8 @@ Definition undef_test13b : list (toplevel_entity typ (list (block typ)))
                         {|
                           blk_id := (Anon 0%Z);
                           blk_phis := [];
-                          blk_code := [(IId (Name "r"), (INSTR_Op (OP_IBinop (LShr false) (TYPE_I 64%Z) (EXP_Ident (ID_Local (Name "a"))) EXP_Undef)))];
-                          blk_term := (IVoid 0%Z, TERM_Ret ((TYPE_I 64%Z), (EXP_Ident (ID_Local (Name "r")))));
+                          blk_code := [(IId (Name "r"), (INSTR_Op (OP_IBinop (LShr false) (TYPE_I 64%N) (EXP_Ident (ID_Local (Name "a"))) EXP_Undef)))];
+                          blk_term := TERM_Ret ((TYPE_I 64%N), (EXP_Ident (ID_Local (Name "r"))));
                           blk_comments := None
                         |}]
         |}].
@@ -900,7 +900,7 @@ Definition undef_test13b : list (toplevel_entity typ (list (block typ)))
 Definition undef_test14 : list (toplevel_entity typ (list (block typ)))
   := [TLE_Definition {|
           df_prototype := {|dc_name := (Name "test14");
-                            dc_type := (TYPE_Function (TYPE_I 1%Z) []);
+                            dc_type := (TYPE_Function (TYPE_I 1%N) []);
                             dc_param_attrs := ([], []);
                             dc_linkage := None;
                             dc_visibility := None;
@@ -915,8 +915,8 @@ Definition undef_test14 : list (toplevel_entity typ (list (block typ)))
                         {|
                           blk_id := (Anon 0%Z);
                           blk_phis := [];
-                          blk_code := [(IId (Name "r"), (INSTR_Op (OP_ICmp Slt (TYPE_I 64%Z) EXP_Undef EXP_Undef)))];
-                          blk_term := (IVoid 0%Z, TERM_Ret ((TYPE_I 1%Z), (EXP_Ident (ID_Local (Name "r")))));
+                          blk_code := [(IId (Name "r"), (INSTR_Op (OP_ICmp Slt (TYPE_I 64%N) EXP_Undef EXP_Undef)))];
+                          blk_term := TERM_Ret ((TYPE_I 1%N), (EXP_Ident (ID_Local (Name "r"))));
                           blk_comments := None
                         |}]
         |}].
@@ -924,7 +924,7 @@ Definition undef_test14 : list (toplevel_entity typ (list (block typ)))
 Definition undef_test15 : list (toplevel_entity typ (list (block typ)))
   := [TLE_Definition {|
           df_prototype := {|dc_name := (Name "test15");
-                            dc_type := (TYPE_Function (TYPE_I 1%Z) []);
+                            dc_type := (TYPE_Function (TYPE_I 1%N) []);
                             dc_param_attrs := ([], []);
                             dc_linkage := None;
                             dc_visibility := None;
@@ -939,8 +939,8 @@ Definition undef_test15 : list (toplevel_entity typ (list (block typ)))
                         {|
                           blk_id := (Anon 0%Z);
                           blk_phis := [];
-                          blk_code := [(IId (Name "r"), (INSTR_Op (OP_ICmp Ult (TYPE_I 64%Z) EXP_Undef EXP_Undef)))];
-                          blk_term := (IVoid 0%Z, TERM_Ret ((TYPE_I 1%Z), (EXP_Ident (ID_Local (Name "r")))));
+                          blk_code := [(IId (Name "r"), (INSTR_Op (OP_ICmp Ult (TYPE_I 64%N) EXP_Undef EXP_Undef)))];
+                          blk_term := TERM_Ret ((TYPE_I 1%N), (EXP_Ident (ID_Local (Name "r"))));
                           blk_comments := None
                         |}]
         |}].
@@ -948,7 +948,7 @@ Definition undef_test15 : list (toplevel_entity typ (list (block typ)))
 Definition undef_test16 : list (toplevel_entity typ (list (block typ)))
   := [TLE_Definition {|
           df_prototype := {|dc_name := (Name "test16");
-                            dc_type := (TYPE_Function (TYPE_I 64%Z) [(TYPE_I 64%Z)]);
+                            dc_type := (TYPE_Function (TYPE_I 64%N) [(TYPE_I 64%N)]);
                             dc_param_attrs := ([], []);
                             dc_linkage := None;
                             dc_visibility := None;
@@ -963,8 +963,8 @@ Definition undef_test16 : list (toplevel_entity typ (list (block typ)))
                         {|
                           blk_id := (Anon 0%Z);
                           blk_phis := [];
-                          blk_code := [(IId (Name "r"), (INSTR_Op (OP_Select ((TYPE_I 1%Z),EXP_Undef) ((TYPE_I 64%Z),(EXP_Ident (ID_Local (Name "a")))) ((TYPE_I 64%Z),EXP_Undef))))];
-                          blk_term := (IVoid 0%Z, TERM_Ret ((TYPE_I 64%Z), (EXP_Ident (ID_Local (Name "r")))));
+                          blk_code := [(IId (Name "r"), (INSTR_Op (OP_Select ((TYPE_I 1%N),EXP_Undef) ((TYPE_I 64%N),(EXP_Ident (ID_Local (Name "a")))) ((TYPE_I 64%N),EXP_Undef))))];
+                          blk_term := TERM_Ret ((TYPE_I 64%N), (EXP_Ident (ID_Local (Name "r"))));
                           blk_comments := None
                         |}]
         |}].
@@ -972,7 +972,7 @@ Definition undef_test16 : list (toplevel_entity typ (list (block typ)))
 Definition undef_test17 : list (toplevel_entity typ (list (block typ)))
   := [TLE_Definition {|
           df_prototype := {|dc_name := (Name "test17");
-                            dc_type := (TYPE_Function (TYPE_I 64%Z) [(TYPE_I 64%Z)]);
+                            dc_type := (TYPE_Function (TYPE_I 64%N) [(TYPE_I 64%N)]);
                             dc_param_attrs := ([], []);
                             dc_linkage := None;
                             dc_visibility := None;
@@ -987,8 +987,8 @@ Definition undef_test17 : list (toplevel_entity typ (list (block typ)))
                         {|
                           blk_id := (Anon 0%Z);
                           blk_phis := [];
-                          blk_code := [(IId (Name "r"), (INSTR_Op (OP_Select ((TYPE_I 1%Z),EXP_Undef) ((TYPE_I 64%Z),EXP_Undef) ((TYPE_I 64%Z),(EXP_Ident (ID_Local (Name "a")))))))];
-                          blk_term := (IVoid 0%Z, TERM_Ret ((TYPE_I 64%Z), (EXP_Ident (ID_Local (Name "r")))));
+                          blk_code := [(IId (Name "r"), (INSTR_Op (OP_Select ((TYPE_I 1%N),EXP_Undef) ((TYPE_I 64%N),EXP_Undef) ((TYPE_I 64%N),(EXP_Ident (ID_Local (Name "a")))))))];
+                          blk_term := TERM_Ret ((TYPE_I 64%N), (EXP_Ident (ID_Local (Name "r"))));
                           blk_comments := None
                         |}]
         |}].
@@ -996,7 +996,7 @@ Definition undef_test17 : list (toplevel_entity typ (list (block typ)))
 Definition undef_test18 : list (toplevel_entity typ (list (block typ)))
   := [TLE_Definition {|
           df_prototype := {|dc_name := (Name "test18");
-                            dc_type := (TYPE_Function (TYPE_I 64%Z) [(TYPE_I 64%Z)]);
+                            dc_type := (TYPE_Function (TYPE_I 64%N) [(TYPE_I 64%N)]);
                             dc_param_attrs := ([], []);
                             dc_linkage := None;
                             dc_visibility := None;
@@ -1011,8 +1011,8 @@ Definition undef_test18 : list (toplevel_entity typ (list (block typ)))
                         {|
                           blk_id := (Anon 0%Z);
                           blk_phis := [];
-                          blk_code := [(IId (Name "r"), (INSTR_Call ((TYPE_Function (TYPE_I 64%Z) [(TYPE_I 64%Z)]), EXP_Undef) [((TYPE_I 64%Z), (EXP_Ident (ID_Local (Name "a"))))]))];
-                          blk_term := (IVoid 0%Z, TERM_Ret ((TYPE_I 64%Z), (EXP_Ident (ID_Local (Name "r")))));
+                          blk_code := [(IId (Name "r"), (INSTR_Call ((TYPE_Function (TYPE_I 64%N) [(TYPE_I 64%N)]), EXP_Undef) [((TYPE_I 64%N), (EXP_Ident (ID_Local (Name "a"))))]))];
+                          blk_term := TERM_Ret ((TYPE_I 64%N), (EXP_Ident (ID_Local (Name "r"))));
                           blk_comments := None
                         |}]
         |}].
@@ -1020,7 +1020,7 @@ Definition undef_test18 : list (toplevel_entity typ (list (block typ)))
 Definition undef_test19 : list (toplevel_entity typ (list (block typ)))
   := [TLE_Definition {|
           df_prototype := {|dc_name := (Name "test19");
-                            dc_type := (TYPE_Function (TYPE_Vector 4%Z (TYPE_I 8%Z)) [(TYPE_Vector 4%Z (TYPE_I 8%Z))]);
+                            dc_type := (TYPE_Function (TYPE_Vector 4%N (TYPE_I 8%N)) [(TYPE_Vector 4%N (TYPE_I 8%N))]);
                             dc_param_attrs := ([], []);
                             dc_linkage := None;
                             dc_visibility := None;
@@ -1035,8 +1035,8 @@ Definition undef_test19 : list (toplevel_entity typ (list (block typ)))
                         {|
                           blk_id := (Anon 0%Z);
                           blk_phis := [];
-                          blk_code := [(IId (Name "b"), (INSTR_Op (OP_IBinop (Shl false false) (TYPE_Vector 4%Z (TYPE_I 8%Z)) (EXP_Ident (ID_Local (Name "a"))) (EXP_Vector [((TYPE_I 8%Z),(EXP_Integer 8%Z)); ((TYPE_I 8%Z),(EXP_Integer 9%Z)); ((TYPE_I 8%Z),EXP_Undef); ((TYPE_I 8%Z), (EXP_Integer (-1)%Z))]))))];
-                          blk_term := (IVoid 0%Z, TERM_Ret ((TYPE_Vector 4%Z (TYPE_I 8%Z)), (EXP_Ident (ID_Local (Name "b")))));
+                          blk_code := [(IId (Name "b"), (INSTR_Op (OP_IBinop (Shl false false) (TYPE_Vector 4%N (TYPE_I 8%N)) (EXP_Ident (ID_Local (Name "a"))) (EXP_Vector [((TYPE_I 8%N),(EXP_Integer 8%Z)); ((TYPE_I 8%N),(EXP_Integer 9%Z)); ((TYPE_I 8%N),EXP_Undef); ((TYPE_I 8%N), (EXP_Integer (-1)%Z))]))))];
+                          blk_term := TERM_Ret ((TYPE_Vector 4%N (TYPE_I 8%N)), (EXP_Ident (ID_Local (Name "b"))));
                           blk_comments := None
                         |}]
         |}].
@@ -1044,7 +1044,7 @@ Definition undef_test19 : list (toplevel_entity typ (list (block typ)))
 Definition undef_test20 : list (toplevel_entity typ (list (block typ)))
   := [TLE_Definition {|
           df_prototype := {|dc_name := (Name "test20");
-                            dc_type := (TYPE_Function (TYPE_I 32%Z) [(TYPE_I 32%Z)]);
+                            dc_type := (TYPE_Function (TYPE_I 32%N) [(TYPE_I 32%N)]);
                             dc_param_attrs := ([], []);
                             dc_linkage := None;
                             dc_visibility := None;
@@ -1059,8 +1059,8 @@ Definition undef_test20 : list (toplevel_entity typ (list (block typ)))
                         {|
                           blk_id := (Anon 0%Z);
                           blk_phis := [];
-                          blk_code := [(IId (Name "b"), (INSTR_Op (OP_IBinop (UDiv false) (TYPE_I 32%Z) (EXP_Ident (ID_Local (Name "a"))) (EXP_Integer 0%Z))))];
-                          blk_term := (IVoid 0%Z, TERM_Ret ((TYPE_I 32%Z), (EXP_Ident (ID_Local (Name "b")))));
+                          blk_code := [(IId (Name "b"), (INSTR_Op (OP_IBinop (UDiv false) (TYPE_I 32%N) (EXP_Ident (ID_Local (Name "a"))) (EXP_Integer 0%Z))))];
+                          blk_term := TERM_Ret ((TYPE_I 32%N), (EXP_Ident (ID_Local (Name "b"))));
                           blk_comments := None
                         |}]
         |}].
@@ -1068,7 +1068,7 @@ Definition undef_test20 : list (toplevel_entity typ (list (block typ)))
 Definition undef_test20vec : list (toplevel_entity typ (list (block typ)))
   := [TLE_Definition {|
           df_prototype := {|dc_name := (Name "test20vec");
-                            dc_type := (TYPE_Function (TYPE_Vector 2%Z (TYPE_I 32%Z)) [(TYPE_Vector 2%Z (TYPE_I 32%Z))]);
+                            dc_type := (TYPE_Function (TYPE_Vector 2%N (TYPE_I 32%N)) [(TYPE_Vector 2%N (TYPE_I 32%N))]);
                             dc_param_attrs := ([], []);
                             dc_linkage := None;
                             dc_visibility := None;
@@ -1083,8 +1083,8 @@ Definition undef_test20vec : list (toplevel_entity typ (list (block typ)))
                         {|
                           blk_id := (Anon 0%Z);
                           blk_phis := [];
-                          blk_code := [(IId (Name "b"), (INSTR_Op (OP_IBinop (UDiv false) (TYPE_Vector 2%Z (TYPE_I 32%Z)) (EXP_Ident (ID_Local (Name "a"))) EXP_Zero_initializer)))];
-                          blk_term := (IVoid 0%Z, TERM_Ret ((TYPE_Vector 2%Z (TYPE_I 32%Z)), (EXP_Ident (ID_Local (Name "b")))));
+                          blk_code := [(IId (Name "b"), (INSTR_Op (OP_IBinop (UDiv false) (TYPE_Vector 2%N (TYPE_I 32%N)) (EXP_Ident (ID_Local (Name "a"))) EXP_Zero_initializer)))];
+                          blk_term := TERM_Ret ((TYPE_Vector 2%N (TYPE_I 32%N)), (EXP_Ident (ID_Local (Name "b"))));
                           blk_comments := None
                         |}]
         |}].
@@ -1092,7 +1092,7 @@ Definition undef_test20vec : list (toplevel_entity typ (list (block typ)))
 Definition undef_test21 : list (toplevel_entity typ (list (block typ)))
   := [TLE_Definition {|
           df_prototype := {|dc_name := (Name "test21");
-                            dc_type := (TYPE_Function (TYPE_I 32%Z) [(TYPE_I 32%Z)]);
+                            dc_type := (TYPE_Function (TYPE_I 32%N) [(TYPE_I 32%N)]);
                             dc_param_attrs := ([], []);
                             dc_linkage := None;
                             dc_visibility := None;
@@ -1107,8 +1107,8 @@ Definition undef_test21 : list (toplevel_entity typ (list (block typ)))
                         {|
                           blk_id := (Anon 0%Z);
                           blk_phis := [];
-                          blk_code := [(IId (Name "b"), (INSTR_Op (OP_IBinop (SDiv false) (TYPE_I 32%Z) (EXP_Ident (ID_Local (Name "a"))) (EXP_Integer 0%Z))))];
-                          blk_term := (IVoid 0%Z, TERM_Ret ((TYPE_I 32%Z), (EXP_Ident (ID_Local (Name "b")))));
+                          blk_code := [(IId (Name "b"), (INSTR_Op (OP_IBinop (SDiv false) (TYPE_I 32%N) (EXP_Ident (ID_Local (Name "a"))) (EXP_Integer 0%Z))))];
+                          blk_term := TERM_Ret ((TYPE_I 32%N), (EXP_Ident (ID_Local (Name "b"))));
                           blk_comments := None
                         |}]
         |}].
@@ -1116,7 +1116,7 @@ Definition undef_test21 : list (toplevel_entity typ (list (block typ)))
 Definition undef_test21vec : list (toplevel_entity typ (list (block typ)))
   := [TLE_Definition {|
           df_prototype := {|dc_name := (Name "test21vec");
-                            dc_type := (TYPE_Function (TYPE_Vector 2%Z (TYPE_I 32%Z)) [(TYPE_Vector 2%Z (TYPE_I 32%Z))]);
+                            dc_type := (TYPE_Function (TYPE_Vector 2%N (TYPE_I 32%N)) [(TYPE_Vector 2%N (TYPE_I 32%N))]);
                             dc_param_attrs := ([], []);
                             dc_linkage := None;
                             dc_visibility := None;
@@ -1131,8 +1131,8 @@ Definition undef_test21vec : list (toplevel_entity typ (list (block typ)))
                         {|
                           blk_id := (Anon 0%Z);
                           blk_phis := [];
-                          blk_code := [(IId (Name "b"), (INSTR_Op (OP_IBinop (SDiv false) (TYPE_Vector 2%Z (TYPE_I 32%Z)) (EXP_Ident (ID_Local (Name "a"))) EXP_Zero_initializer)))];
-                          blk_term := (IVoid 0%Z, TERM_Ret ((TYPE_Vector 2%Z (TYPE_I 32%Z)), (EXP_Ident (ID_Local (Name "b")))));
+                          blk_code := [(IId (Name "b"), (INSTR_Op (OP_IBinop (SDiv false) (TYPE_Vector 2%N (TYPE_I 32%N)) (EXP_Ident (ID_Local (Name "a"))) EXP_Zero_initializer)))];
+                          blk_term := TERM_Ret ((TYPE_Vector 2%N (TYPE_I 32%N)), (EXP_Ident (ID_Local (Name "b"))));
                           blk_comments := None
                         |}]
         |}].
@@ -1140,7 +1140,7 @@ Definition undef_test21vec : list (toplevel_entity typ (list (block typ)))
 Definition undef_test22 : list (toplevel_entity typ (list (block typ)))
   := [TLE_Definition {|
           df_prototype := {|dc_name := (Name "test22");
-                            dc_type := (TYPE_Function (TYPE_I 32%Z) [(TYPE_I 32%Z)]);
+                            dc_type := (TYPE_Function (TYPE_I 32%N) [(TYPE_I 32%N)]);
                             dc_param_attrs := ([], []);
                             dc_linkage := None;
                             dc_visibility := None;
@@ -1155,8 +1155,8 @@ Definition undef_test22 : list (toplevel_entity typ (list (block typ)))
                         {|
                           blk_id := (Anon 0%Z);
                           blk_phis := [];
-                          blk_code := [(IId (Name "b"), (INSTR_Op (OP_IBinop (AShr true) (TYPE_I 32%Z) EXP_Undef (EXP_Ident (ID_Local (Name "a"))))))];
-                          blk_term := (IVoid 0%Z, TERM_Ret ((TYPE_I 32%Z), (EXP_Ident (ID_Local (Name "b")))));
+                          blk_code := [(IId (Name "b"), (INSTR_Op (OP_IBinop (AShr true) (TYPE_I 32%N) EXP_Undef (EXP_Ident (ID_Local (Name "a"))))))];
+                          blk_term := TERM_Ret ((TYPE_I 32%N), (EXP_Ident (ID_Local (Name "b"))));
                           blk_comments := None
                         |}]
         |}].
@@ -1164,7 +1164,7 @@ Definition undef_test22 : list (toplevel_entity typ (list (block typ)))
 Definition undef_test23 : list (toplevel_entity typ (list (block typ)))
   := [TLE_Definition {|
           df_prototype := {|dc_name := (Name "test23");
-                            dc_type := (TYPE_Function (TYPE_I 32%Z) [(TYPE_I 32%Z)]);
+                            dc_type := (TYPE_Function (TYPE_I 32%N) [(TYPE_I 32%N)]);
                             dc_param_attrs := ([], []);
                             dc_linkage := None;
                             dc_visibility := None;
@@ -1179,8 +1179,8 @@ Definition undef_test23 : list (toplevel_entity typ (list (block typ)))
                         {|
                           blk_id := (Anon 0%Z);
                           blk_phis := [];
-                          blk_code := [(IId (Name "b"), (INSTR_Op (OP_IBinop (LShr true) (TYPE_I 32%Z) EXP_Undef (EXP_Ident (ID_Local (Name "a"))))))];
-                          blk_term := (IVoid 0%Z, TERM_Ret ((TYPE_I 32%Z), (EXP_Ident (ID_Local (Name "b")))));
+                          blk_code := [(IId (Name "b"), (INSTR_Op (OP_IBinop (LShr true) (TYPE_I 32%N) EXP_Undef (EXP_Ident (ID_Local (Name "a"))))))];
+                          blk_term := TERM_Ret ((TYPE_I 32%N), (EXP_Ident (ID_Local (Name "b"))));
                           blk_comments := None
                         |}]
         |}].
@@ -1188,7 +1188,7 @@ Definition undef_test23 : list (toplevel_entity typ (list (block typ)))
 Definition undef_test24 : list (toplevel_entity typ (list (block typ)))
   := [TLE_Definition {|
           df_prototype := {|dc_name := (Name "test24");
-                            dc_type := (TYPE_Function (TYPE_I 32%Z) []);
+                            dc_type := (TYPE_Function (TYPE_I 32%N) []);
                             dc_param_attrs := ([], []);
                             dc_linkage := None;
                             dc_visibility := None;
@@ -1203,8 +1203,8 @@ Definition undef_test24 : list (toplevel_entity typ (list (block typ)))
                         {|
                           blk_id := (Anon 0%Z);
                           blk_phis := [];
-                          blk_code := [(IId (Name "b"), (INSTR_Op (OP_IBinop (UDiv false) (TYPE_I 32%Z) EXP_Undef (EXP_Integer 0%Z))))];
-                          blk_term := (IVoid 0%Z, TERM_Ret ((TYPE_I 32%Z), (EXP_Ident (ID_Local (Name "b")))));
+                          blk_code := [(IId (Name "b"), (INSTR_Op (OP_IBinop (UDiv false) (TYPE_I 32%N) EXP_Undef (EXP_Integer 0%Z))))];
+                          blk_term := TERM_Ret ((TYPE_I 32%N), (EXP_Ident (ID_Local (Name "b"))));
                           blk_comments := None
                         |}]
         |}].
@@ -1212,7 +1212,7 @@ Definition undef_test24 : list (toplevel_entity typ (list (block typ)))
 Definition undef_test25 : list (toplevel_entity typ (list (block typ)))
   := [TLE_Definition {|
           df_prototype := {|dc_name := (Name "test25");
-                            dc_type := (TYPE_Function (TYPE_I 32%Z) []);
+                            dc_type := (TYPE_Function (TYPE_I 32%N) []);
                             dc_param_attrs := ([], []);
                             dc_linkage := None;
                             dc_visibility := None;
@@ -1227,8 +1227,8 @@ Definition undef_test25 : list (toplevel_entity typ (list (block typ)))
                         {|
                           blk_id := (Anon 0%Z);
                           blk_phis := [];
-                          blk_code := [(IId (Name "b"), (INSTR_Op (OP_IBinop (LShr false) (TYPE_I 32%Z) (EXP_Integer 0%Z) EXP_Undef)))];
-                          blk_term := (IVoid 0%Z, TERM_Ret ((TYPE_I 32%Z), (EXP_Ident (ID_Local (Name "b")))));
+                          blk_code := [(IId (Name "b"), (INSTR_Op (OP_IBinop (LShr false) (TYPE_I 32%N) (EXP_Integer 0%Z) EXP_Undef)))];
+                          blk_term := TERM_Ret ((TYPE_I 32%N), (EXP_Ident (ID_Local (Name "b"))));
                           blk_comments := None
                         |}]
         |}].
@@ -1236,7 +1236,7 @@ Definition undef_test25 : list (toplevel_entity typ (list (block typ)))
 Definition undef_test26 : list (toplevel_entity typ (list (block typ)))
   := [TLE_Definition {|
           df_prototype := {|dc_name := (Name "test26");
-                            dc_type := (TYPE_Function (TYPE_I 32%Z) []);
+                            dc_type := (TYPE_Function (TYPE_I 32%N) []);
                             dc_param_attrs := ([], []);
                             dc_linkage := None;
                             dc_visibility := None;
@@ -1251,8 +1251,8 @@ Definition undef_test26 : list (toplevel_entity typ (list (block typ)))
                         {|
                           blk_id := (Anon 0%Z);
                           blk_phis := [];
-                          blk_code := [(IId (Name "b"), (INSTR_Op (OP_IBinop (AShr false) (TYPE_I 32%Z) (EXP_Integer 0%Z) EXP_Undef)))];
-                          blk_term := (IVoid 0%Z, TERM_Ret ((TYPE_I 32%Z), (EXP_Ident (ID_Local (Name "b")))));
+                          blk_code := [(IId (Name "b"), (INSTR_Op (OP_IBinop (AShr false) (TYPE_I 32%N) (EXP_Integer 0%Z) EXP_Undef)))];
+                          blk_term := TERM_Ret ((TYPE_I 32%N), (EXP_Ident (ID_Local (Name "b"))));
                           blk_comments := None
                         |}]
         |}].
@@ -1260,7 +1260,7 @@ Definition undef_test26 : list (toplevel_entity typ (list (block typ)))
 Definition undef_test27 : list (toplevel_entity typ (list (block typ)))
   := [TLE_Definition {|
           df_prototype := {|dc_name := (Name "test27");
-                            dc_type := (TYPE_Function (TYPE_I 32%Z) []);
+                            dc_type := (TYPE_Function (TYPE_I 32%N) []);
                             dc_param_attrs := ([], []);
                             dc_linkage := None;
                             dc_visibility := None;
@@ -1275,8 +1275,8 @@ Definition undef_test27 : list (toplevel_entity typ (list (block typ)))
                         {|
                           blk_id := (Anon 0%Z);
                           blk_phis := [];
-                          blk_code := [(IId (Name "b"), (INSTR_Op (OP_IBinop (Shl false false) (TYPE_I 32%Z) (EXP_Integer 0%Z) EXP_Undef)))];
-                          blk_term := (IVoid 0%Z, TERM_Ret ((TYPE_I 32%Z), (EXP_Ident (ID_Local (Name "b")))));
+                          blk_code := [(IId (Name "b"), (INSTR_Op (OP_IBinop (Shl false false) (TYPE_I 32%N) (EXP_Integer 0%Z) EXP_Undef)))];
+                          blk_term := TERM_Ret ((TYPE_I 32%N), (EXP_Ident (ID_Local (Name "b"))));
                           blk_comments := None
                         |}]
         |}].
@@ -1284,7 +1284,7 @@ Definition undef_test27 : list (toplevel_entity typ (list (block typ)))
 Definition undef_test28 : list (toplevel_entity typ (list (block typ)))
   := [TLE_Definition {|
           df_prototype := {|dc_name := (Name "test28");
-                            dc_type := (TYPE_Function (TYPE_I 32%Z) [(TYPE_I 32%Z)]);
+                            dc_type := (TYPE_Function (TYPE_I 32%N) [(TYPE_I 32%N)]);
                             dc_param_attrs := ([], []);
                             dc_linkage := None;
                             dc_visibility := None;
@@ -1299,8 +1299,8 @@ Definition undef_test28 : list (toplevel_entity typ (list (block typ)))
                         {|
                           blk_id := (Anon 0%Z);
                           blk_phis := [];
-                          blk_code := [(IId (Name "b"), (INSTR_Op (OP_IBinop (Shl false true) (TYPE_I 32%Z) EXP_Undef (EXP_Ident (ID_Local (Name "a"))))))];
-                          blk_term := (IVoid 0%Z, TERM_Ret ((TYPE_I 32%Z), (EXP_Ident (ID_Local (Name "b")))));
+                          blk_code := [(IId (Name "b"), (INSTR_Op (OP_IBinop (Shl false true) (TYPE_I 32%N) EXP_Undef (EXP_Ident (ID_Local (Name "a"))))))];
+                          blk_term := TERM_Ret ((TYPE_I 32%N), (EXP_Ident (ID_Local (Name "b"))));
                           blk_comments := None
                         |}]
         |}].
@@ -1308,7 +1308,7 @@ Definition undef_test28 : list (toplevel_entity typ (list (block typ)))
 Definition undef_test29 : list (toplevel_entity typ (list (block typ)))
   := [TLE_Definition {|
           df_prototype := {|dc_name := (Name "test29");
-                            dc_type := (TYPE_Function (TYPE_I 32%Z) [(TYPE_I 32%Z)]);
+                            dc_type := (TYPE_Function (TYPE_I 32%N) [(TYPE_I 32%N)]);
                             dc_param_attrs := ([], []);
                             dc_linkage := None;
                             dc_visibility := None;
@@ -1323,8 +1323,8 @@ Definition undef_test29 : list (toplevel_entity typ (list (block typ)))
                         {|
                           blk_id := (Anon 0%Z);
                           blk_phis := [];
-                          blk_code := [(IId (Name "b"), (INSTR_Op (OP_IBinop (Shl true false) (TYPE_I 32%Z) EXP_Undef (EXP_Ident (ID_Local (Name "a"))))))];
-                          blk_term := (IVoid 0%Z, TERM_Ret ((TYPE_I 32%Z), (EXP_Ident (ID_Local (Name "b")))));
+                          blk_code := [(IId (Name "b"), (INSTR_Op (OP_IBinop (Shl true false) (TYPE_I 32%N) EXP_Undef (EXP_Ident (ID_Local (Name "a"))))))];
+                          blk_term := TERM_Ret ((TYPE_I 32%N), (EXP_Ident (ID_Local (Name "b"))));
                           blk_comments := None
                         |}]
         |}].
@@ -1332,7 +1332,7 @@ Definition undef_test29 : list (toplevel_entity typ (list (block typ)))
 Definition undef_test30 : list (toplevel_entity typ (list (block typ)))
   := [TLE_Definition {|
           df_prototype := {|dc_name := (Name "test30");
-                            dc_type := (TYPE_Function (TYPE_I 32%Z) [(TYPE_I 32%Z)]);
+                            dc_type := (TYPE_Function (TYPE_I 32%N) [(TYPE_I 32%N)]);
                             dc_param_attrs := ([], []);
                             dc_linkage := None;
                             dc_visibility := None;
@@ -1347,8 +1347,8 @@ Definition undef_test30 : list (toplevel_entity typ (list (block typ)))
                         {|
                           blk_id := (Anon 0%Z);
                           blk_phis := [];
-                          blk_code := [(IId (Name "b"), (INSTR_Op (OP_IBinop (Shl true true) (TYPE_I 32%Z) EXP_Undef (EXP_Ident (ID_Local (Name "a"))))))];
-                          blk_term := (IVoid 0%Z, TERM_Ret ((TYPE_I 32%Z), (EXP_Ident (ID_Local (Name "b")))));
+                          blk_code := [(IId (Name "b"), (INSTR_Op (OP_IBinop (Shl true true) (TYPE_I 32%N) EXP_Undef (EXP_Ident (ID_Local (Name "a"))))))];
+                          blk_term := TERM_Ret ((TYPE_I 32%N), (EXP_Ident (ID_Local (Name "b"))));
                           blk_comments := None
                         |}]
         |}].
@@ -1356,7 +1356,7 @@ Definition undef_test30 : list (toplevel_entity typ (list (block typ)))
 Definition undef_test31 : list (toplevel_entity typ (list (block typ)))
   := [TLE_Definition {|
           df_prototype := {|dc_name := (Name "test31");
-                            dc_type := (TYPE_Function (TYPE_I 32%Z) [(TYPE_I 32%Z)]);
+                            dc_type := (TYPE_Function (TYPE_I 32%N) [(TYPE_I 32%N)]);
                             dc_param_attrs := ([], []);
                             dc_linkage := None;
                             dc_visibility := None;
@@ -1371,8 +1371,8 @@ Definition undef_test31 : list (toplevel_entity typ (list (block typ)))
                         {|
                           blk_id := (Anon 0%Z);
                           blk_phis := [];
-                          blk_code := [(IId (Name "b"), (INSTR_Op (OP_IBinop (Shl false false) (TYPE_I 32%Z) EXP_Undef (EXP_Ident (ID_Local (Name "a"))))))];
-                          blk_term := (IVoid 0%Z, TERM_Ret ((TYPE_I 32%Z), (EXP_Ident (ID_Local (Name "b")))));
+                          blk_code := [(IId (Name "b"), (INSTR_Op (OP_IBinop (Shl false false) (TYPE_I 32%N) EXP_Undef (EXP_Ident (ID_Local (Name "a"))))))];
+                          blk_term := TERM_Ret ((TYPE_I 32%N), (EXP_Ident (ID_Local (Name "b"))));
                           blk_comments := None
                         |}]
         |}].
@@ -1380,7 +1380,7 @@ Definition undef_test31 : list (toplevel_entity typ (list (block typ)))
 Definition undef_test32 : list (toplevel_entity typ (list (block typ)))
   := [TLE_Definition {|
           df_prototype := {|dc_name := (Name "test32");
-                            dc_type := (TYPE_Function (TYPE_I 32%Z) [(TYPE_I 32%Z)]);
+                            dc_type := (TYPE_Function (TYPE_I 32%N) [(TYPE_I 32%N)]);
                             dc_param_attrs := ([], []);
                             dc_linkage := None;
                             dc_visibility := None;
@@ -1395,8 +1395,8 @@ Definition undef_test32 : list (toplevel_entity typ (list (block typ)))
                         {|
                           blk_id := (Anon 0%Z);
                           blk_phis := [];
-                          blk_code := [(IId (Name "b"), (INSTR_Op (OP_IBinop (Shl false false) (TYPE_I 32%Z) EXP_Undef (EXP_Integer 0%Z))))];
-                          blk_term := (IVoid 0%Z, TERM_Ret ((TYPE_I 32%Z), (EXP_Ident (ID_Local (Name "b")))));
+                          blk_code := [(IId (Name "b"), (INSTR_Op (OP_IBinop (Shl false false) (TYPE_I 32%N) EXP_Undef (EXP_Integer 0%Z))))];
+                          blk_term := TERM_Ret ((TYPE_I 32%N), (EXP_Ident (ID_Local (Name "b"))));
                           blk_comments := None
                         |}]
         |}].
@@ -1404,7 +1404,7 @@ Definition undef_test32 : list (toplevel_entity typ (list (block typ)))
 Definition undef_test33 : list (toplevel_entity typ (list (block typ)))
   := [TLE_Definition {|
           df_prototype := {|dc_name := (Name "test33");
-                            dc_type := (TYPE_Function (TYPE_I 32%Z) [(TYPE_I 32%Z)]);
+                            dc_type := (TYPE_Function (TYPE_I 32%N) [(TYPE_I 32%N)]);
                             dc_param_attrs := ([], []);
                             dc_linkage := None;
                             dc_visibility := None;
@@ -1419,8 +1419,8 @@ Definition undef_test33 : list (toplevel_entity typ (list (block typ)))
                         {|
                           blk_id := (Anon 0%Z);
                           blk_phis := [];
-                          blk_code := [(IId (Name "b"), (INSTR_Op (OP_IBinop (AShr false) (TYPE_I 32%Z) EXP_Undef (EXP_Integer 0%Z))))];
-                          blk_term := (IVoid 0%Z, TERM_Ret ((TYPE_I 32%Z), (EXP_Ident (ID_Local (Name "b")))));
+                          blk_code := [(IId (Name "b"), (INSTR_Op (OP_IBinop (AShr false) (TYPE_I 32%N) EXP_Undef (EXP_Integer 0%Z))))];
+                          blk_term := TERM_Ret ((TYPE_I 32%N), (EXP_Ident (ID_Local (Name "b"))));
                           blk_comments := None
                         |}]
         |}].
@@ -1428,7 +1428,7 @@ Definition undef_test33 : list (toplevel_entity typ (list (block typ)))
 Definition undef_test34 : list (toplevel_entity typ (list (block typ)))
   := [TLE_Definition {|
           df_prototype := {|dc_name := (Name "test34");
-                            dc_type := (TYPE_Function (TYPE_I 32%Z) [(TYPE_I 32%Z)]);
+                            dc_type := (TYPE_Function (TYPE_I 32%N) [(TYPE_I 32%N)]);
                             dc_param_attrs := ([], []);
                             dc_linkage := None;
                             dc_visibility := None;
@@ -1443,8 +1443,8 @@ Definition undef_test34 : list (toplevel_entity typ (list (block typ)))
                         {|
                           blk_id := (Anon 0%Z);
                           blk_phis := [];
-                          blk_code := [(IId (Name "b"), (INSTR_Op (OP_IBinop (LShr false) (TYPE_I 32%Z) EXP_Undef (EXP_Integer 0%Z))))];
-                          blk_term := (IVoid 0%Z, TERM_Ret ((TYPE_I 32%Z), (EXP_Ident (ID_Local (Name "b")))));
+                          blk_code := [(IId (Name "b"), (INSTR_Op (OP_IBinop (LShr false) (TYPE_I 32%N) EXP_Undef (EXP_Integer 0%Z))))];
+                          blk_term := TERM_Ret ((TYPE_I 32%N), (EXP_Ident (ID_Local (Name "b"))));
                           blk_comments := None
                         |}]
         |}].
@@ -1452,7 +1452,7 @@ Definition undef_test34 : list (toplevel_entity typ (list (block typ)))
 Definition undef_test35 : list (toplevel_entity typ (list (block typ)))
   := [TLE_Definition {|
           df_prototype := {|dc_name := (Name "test35");
-                            dc_type := (TYPE_Function (TYPE_I 32%Z) [(TYPE_Vector 4%Z (TYPE_I 32%Z))]);
+                            dc_type := (TYPE_Function (TYPE_I 32%N) [(TYPE_Vector 4%N (TYPE_I 32%N))]);
                             dc_param_attrs := ([], []);
                             dc_linkage := None;
                             dc_visibility := None;
@@ -1467,8 +1467,8 @@ Definition undef_test35 : list (toplevel_entity typ (list (block typ)))
                         {|
                           blk_id := (Anon 0%Z);
                           blk_phis := [];
-                          blk_code := [(IId (Name "b"), (INSTR_Op (OP_ExtractElement ((TYPE_Vector 4%Z (TYPE_I 32%Z)),(EXP_Ident (ID_Local (Name "V")))) ((TYPE_I 32%Z),(EXP_Integer 4%Z)))))];
-                          blk_term := (IVoid 0%Z, TERM_Ret ((TYPE_I 32%Z), (EXP_Ident (ID_Local (Name "b")))));
+                          blk_code := [(IId (Name "b"), (INSTR_Op (OP_ExtractElement ((TYPE_Vector 4%N (TYPE_I 32%N)),(EXP_Ident (ID_Local (Name "V")))) ((TYPE_I 32%N),(EXP_Integer 4%Z)))))];
+                          blk_term := TERM_Ret ((TYPE_I 32%N), (EXP_Ident (ID_Local (Name "b"))));
                           blk_comments := None
                         |}]
         |}].
@@ -1476,7 +1476,7 @@ Definition undef_test35 : list (toplevel_entity typ (list (block typ)))
 Definition undef_test36 : list (toplevel_entity typ (list (block typ)))
   := [TLE_Definition {|
           df_prototype := {|dc_name := (Name "test36");
-                            dc_type := (TYPE_Function (TYPE_I 32%Z) [(TYPE_I 32%Z)]);
+                            dc_type := (TYPE_Function (TYPE_I 32%N) [(TYPE_I 32%N)]);
                             dc_param_attrs := ([], []);
                             dc_linkage := None;
                             dc_visibility := None;
@@ -1491,8 +1491,8 @@ Definition undef_test36 : list (toplevel_entity typ (list (block typ)))
                         {|
                           blk_id := (Anon 0%Z);
                           blk_phis := [];
-                          blk_code := [(IId (Name "b"), (INSTR_Op (OP_ExtractElement ((TYPE_Vector 4%Z (TYPE_I 32%Z)),EXP_Undef) ((TYPE_I 32%Z),(EXP_Ident (ID_Local (Name "V")))))))];
-                          blk_term := (IVoid 0%Z, TERM_Ret ((TYPE_I 32%Z), (EXP_Ident (ID_Local (Name "b")))));
+                          blk_code := [(IId (Name "b"), (INSTR_Op (OP_ExtractElement ((TYPE_Vector 4%N (TYPE_I 32%N)),EXP_Undef) ((TYPE_I 32%N),(EXP_Ident (ID_Local (Name "V")))))))];
+                          blk_term := TERM_Ret ((TYPE_I 32%N), (EXP_Ident (ID_Local (Name "b"))));
                           blk_comments := None
                         |}]
         |}].
@@ -1500,7 +1500,7 @@ Definition undef_test36 : list (toplevel_entity typ (list (block typ)))
 Definition undef_test37 : list (toplevel_entity typ (list (block typ)))
   := [TLE_Definition {|
           df_prototype := {|dc_name := (Name "test37");
-                            dc_type := (TYPE_Function (TYPE_I 32%Z) []);
+                            dc_type := (TYPE_Function (TYPE_I 32%N) []);
                             dc_param_attrs := ([], []);
                             dc_linkage := None;
                             dc_visibility := None;
@@ -1515,8 +1515,8 @@ Definition undef_test37 : list (toplevel_entity typ (list (block typ)))
                         {|
                           blk_id := (Anon 0%Z);
                           blk_phis := [];
-                          blk_code := [(IId (Name "b"), (INSTR_Op (OP_IBinop (UDiv false) (TYPE_I 32%Z) EXP_Undef EXP_Undef)))];
-                          blk_term := (IVoid 0%Z, TERM_Ret ((TYPE_I 32%Z), (EXP_Ident (ID_Local (Name "b")))));
+                          blk_code := [(IId (Name "b"), (INSTR_Op (OP_IBinop (UDiv false) (TYPE_I 32%N) EXP_Undef EXP_Undef)))];
+                          blk_term := TERM_Ret ((TYPE_I 32%N), (EXP_Ident (ID_Local (Name "b"))));
                           blk_comments := None
                         |}]
         |}].
@@ -1524,7 +1524,7 @@ Definition undef_test37 : list (toplevel_entity typ (list (block typ)))
 Definition undef_test38 : list (toplevel_entity typ (list (block typ)))
   := [TLE_Definition {|
           df_prototype := {|dc_name := (Name "test38");
-                            dc_type := (TYPE_Function (TYPE_I 32%Z) [(TYPE_I 32%Z)]);
+                            dc_type := (TYPE_Function (TYPE_I 32%N) [(TYPE_I 32%N)]);
                             dc_param_attrs := ([], []);
                             dc_linkage := None;
                             dc_visibility := None;
@@ -1539,8 +1539,8 @@ Definition undef_test38 : list (toplevel_entity typ (list (block typ)))
                         {|
                           blk_id := (Anon 0%Z);
                           blk_phis := [];
-                          blk_code := [(IId (Name "b"), (INSTR_Op (OP_IBinop (UDiv false) (TYPE_I 32%Z) (EXP_Ident (ID_Local (Name "a"))) EXP_Undef)))];
-                          blk_term := (IVoid 0%Z, TERM_Ret ((TYPE_I 32%Z), (EXP_Ident (ID_Local (Name "b")))));
+                          blk_code := [(IId (Name "b"), (INSTR_Op (OP_IBinop (UDiv false) (TYPE_I 32%N) (EXP_Ident (ID_Local (Name "a"))) EXP_Undef)))];
+                          blk_term := TERM_Ret ((TYPE_I 32%N), (EXP_Ident (ID_Local (Name "b"))));
                           blk_comments := None
                         |}]
         |}].
@@ -1548,7 +1548,7 @@ Definition undef_test38 : list (toplevel_entity typ (list (block typ)))
 Definition undef_test39 : list (toplevel_entity typ (list (block typ)))
   := [TLE_Definition {|
           df_prototype := {|dc_name := (Name "test39");
-                            dc_type := (TYPE_Function (TYPE_I 32%Z) []);
+                            dc_type := (TYPE_Function (TYPE_I 32%N) []);
                             dc_param_attrs := ([], []);
                             dc_linkage := None;
                             dc_visibility := None;
@@ -1563,8 +1563,8 @@ Definition undef_test39 : list (toplevel_entity typ (list (block typ)))
                         {|
                           blk_id := (Anon 0%Z);
                           blk_phis := [];
-                          blk_code := [(IId (Name "b"), (INSTR_Op (OP_IBinop (UDiv false) (TYPE_I 32%Z) (EXP_Integer 0%Z) EXP_Undef)))];
-                          blk_term := (IVoid 0%Z, TERM_Ret ((TYPE_I 32%Z), (EXP_Ident (ID_Local (Name "b")))));
+                          blk_code := [(IId (Name "b"), (INSTR_Op (OP_IBinop (UDiv false) (TYPE_I 32%N) (EXP_Integer 0%Z) EXP_Undef)))];
+                          blk_term := TERM_Ret ((TYPE_I 32%N), (EXP_Ident (ID_Local (Name "b"))));
                           blk_comments := None
                         |}]
         |}].
@@ -1573,7 +1573,7 @@ Definition undef_test39 : list (toplevel_entity typ (list (block typ)))
 Definition undef_tests : list (toplevel_entity typ (list (block typ)))
   := [TLE_Definition {|
   df_prototype := {|dc_name := (Name "test0");
-                    dc_type := (TYPE_Function (TYPE_I 64%Z) []);
+                    dc_type := (TYPE_Function (TYPE_I 64%N) []);
                     dc_param_attrs := ([], []);
                     dc_linkage := None;
                     dc_visibility := None;
@@ -1588,14 +1588,14 @@ Definition undef_tests : list (toplevel_entity typ (list (block typ)))
                 {|
                   blk_id := (Anon 0%Z);
                   blk_phis := [];
-                  blk_code := [(IId (Name "r"), (INSTR_Op (OP_IBinop (Mul false false) (TYPE_I 64%Z) EXP_Undef EXP_Undef)))];
-                  blk_term := (IVoid 0%Z, TERM_Ret ((TYPE_I 64%Z), (EXP_Ident (ID_Local (Name "r")))));
+                  blk_code := [(IId (Name "r"), (INSTR_Op (OP_IBinop (Mul false false) (TYPE_I 64%N) EXP_Undef EXP_Undef)))];
+                  blk_term := TERM_Ret ((TYPE_I 64%N), (EXP_Ident (ID_Local (Name "r"))));
                   blk_comments := None
                 |}]
                 |}; 
 TLE_Definition {|
   df_prototype := {|dc_name := (Name "test1");
-                    dc_type := (TYPE_Function (TYPE_I 64%Z) []);
+                    dc_type := (TYPE_Function (TYPE_I 64%N) []);
                     dc_param_attrs := ([], []);
                     dc_linkage := None;
                     dc_visibility := None;
@@ -1610,14 +1610,14 @@ TLE_Definition {|
                 {|
                   blk_id := (Anon 0%Z);
                   blk_phis := [];
-                  blk_code := [(IId (Name "r"), (INSTR_Op (OP_IBinop (Mul false false) (TYPE_I 64%Z) (EXP_Integer 3%Z) EXP_Undef)))];
-                  blk_term := (IVoid 0%Z, TERM_Ret ((TYPE_I 64%Z), (EXP_Ident (ID_Local (Name "r")))));
+                  blk_code := [(IId (Name "r"), (INSTR_Op (OP_IBinop (Mul false false) (TYPE_I 64%N) (EXP_Integer 3%Z) EXP_Undef)))];
+                  blk_term := TERM_Ret ((TYPE_I 64%N), (EXP_Ident (ID_Local (Name "r"))));
                   blk_comments := None
                 |}]
                 |}; 
 TLE_Definition {|
   df_prototype := {|dc_name := (Name "test2");
-                    dc_type := (TYPE_Function (TYPE_I 64%Z) []);
+                    dc_type := (TYPE_Function (TYPE_I 64%N) []);
                     dc_param_attrs := ([], []);
                     dc_linkage := None;
                     dc_visibility := None;
@@ -1632,14 +1632,14 @@ TLE_Definition {|
                 {|
                   blk_id := (Anon 0%Z);
                   blk_phis := [];
-                  blk_code := [(IId (Name "r"), (INSTR_Op (OP_IBinop (Mul false false) (TYPE_I 64%Z) EXP_Undef (EXP_Integer 3%Z))))];
-                  blk_term := (IVoid 0%Z, TERM_Ret ((TYPE_I 64%Z), (EXP_Ident (ID_Local (Name "r")))));
+                  blk_code := [(IId (Name "r"), (INSTR_Op (OP_IBinop (Mul false false) (TYPE_I 64%N) EXP_Undef (EXP_Integer 3%Z))))];
+                  blk_term := TERM_Ret ((TYPE_I 64%N), (EXP_Ident (ID_Local (Name "r"))));
                   blk_comments := None
                 |}]
                 |}; 
 TLE_Definition {|
   df_prototype := {|dc_name := (Name "test3");
-                    dc_type := (TYPE_Function (TYPE_I 64%Z) []);
+                    dc_type := (TYPE_Function (TYPE_I 64%N) []);
                     dc_param_attrs := ([], []);
                     dc_linkage := None;
                     dc_visibility := None;
@@ -1654,14 +1654,14 @@ TLE_Definition {|
                 {|
                   blk_id := (Anon 0%Z);
                   blk_phis := [];
-                  blk_code := [(IId (Name "r"), (INSTR_Op (OP_IBinop (Mul false false) (TYPE_I 64%Z) EXP_Undef (EXP_Integer 6%Z))))];
-                  blk_term := (IVoid 0%Z, TERM_Ret ((TYPE_I 64%Z), (EXP_Ident (ID_Local (Name "r")))));
+                  blk_code := [(IId (Name "r"), (INSTR_Op (OP_IBinop (Mul false false) (TYPE_I 64%N) EXP_Undef (EXP_Integer 6%Z))))];
+                  blk_term := TERM_Ret ((TYPE_I 64%N), (EXP_Ident (ID_Local (Name "r"))));
                   blk_comments := None
                 |}]
                 |}; 
 TLE_Definition {|
   df_prototype := {|dc_name := (Name "test4");
-                    dc_type := (TYPE_Function (TYPE_I 64%Z) []);
+                    dc_type := (TYPE_Function (TYPE_I 64%N) []);
                     dc_param_attrs := ([], []);
                     dc_linkage := None;
                     dc_visibility := None;
@@ -1676,14 +1676,14 @@ TLE_Definition {|
                 {|
                   blk_id := (Anon 0%Z);
                   blk_phis := [];
-                  blk_code := [(IId (Name "r"), (INSTR_Op (OP_IBinop (Mul false false) (TYPE_I 64%Z) (EXP_Integer 6%Z) EXP_Undef)))];
-                  blk_term := (IVoid 0%Z, TERM_Ret ((TYPE_I 64%Z), (EXP_Ident (ID_Local (Name "r")))));
+                  blk_code := [(IId (Name "r"), (INSTR_Op (OP_IBinop (Mul false false) (TYPE_I 64%N) (EXP_Integer 6%Z) EXP_Undef)))];
+                  blk_term := TERM_Ret ((TYPE_I 64%N), (EXP_Ident (ID_Local (Name "r"))));
                   blk_comments := None
                 |}]
                 |}; 
 TLE_Definition {|
   df_prototype := {|dc_name := (Name "test5");
-                    dc_type := (TYPE_Function (TYPE_I 64%Z) []);
+                    dc_type := (TYPE_Function (TYPE_I 64%N) []);
                     dc_param_attrs := ([], []);
                     dc_linkage := None;
                     dc_visibility := None;
@@ -1698,14 +1698,14 @@ TLE_Definition {|
                 {|
                   blk_id := (Anon 0%Z);
                   blk_phis := [];
-                  blk_code := [(IId (Name "r"), (INSTR_Op (OP_IBinop And (TYPE_I 64%Z) EXP_Undef EXP_Undef)))];
-                  blk_term := (IVoid 0%Z, TERM_Ret ((TYPE_I 64%Z), (EXP_Ident (ID_Local (Name "r")))));
+                  blk_code := [(IId (Name "r"), (INSTR_Op (OP_IBinop And (TYPE_I 64%N) EXP_Undef EXP_Undef)))];
+                  blk_term := TERM_Ret ((TYPE_I 64%N), (EXP_Ident (ID_Local (Name "r"))));
                   blk_comments := None
                 |}]
                 |}; 
 TLE_Definition {|
   df_prototype := {|dc_name := (Name "test6");
-                    dc_type := (TYPE_Function (TYPE_I 64%Z) []);
+                    dc_type := (TYPE_Function (TYPE_I 64%N) []);
                     dc_param_attrs := ([], []);
                     dc_linkage := None;
                     dc_visibility := None;
@@ -1720,14 +1720,14 @@ TLE_Definition {|
                 {|
                   blk_id := (Anon 0%Z);
                   blk_phis := [];
-                  blk_code := [(IId (Name "r"), (INSTR_Op (OP_IBinop Or (TYPE_I 64%Z) EXP_Undef EXP_Undef)))];
-                  blk_term := (IVoid 0%Z, TERM_Ret ((TYPE_I 64%Z), (EXP_Ident (ID_Local (Name "r")))));
+                  blk_code := [(IId (Name "r"), (INSTR_Op (OP_IBinop Or (TYPE_I 64%N) EXP_Undef EXP_Undef)))];
+                  blk_term := TERM_Ret ((TYPE_I 64%N), (EXP_Ident (ID_Local (Name "r"))));
                   blk_comments := None
                 |}]
                 |}; 
 TLE_Definition {|
   df_prototype := {|dc_name := (Name "test7");
-                    dc_type := (TYPE_Function (TYPE_I 64%Z) []);
+                    dc_type := (TYPE_Function (TYPE_I 64%N) []);
                     dc_param_attrs := ([], []);
                     dc_linkage := None;
                     dc_visibility := None;
@@ -1742,14 +1742,14 @@ TLE_Definition {|
                 {|
                   blk_id := (Anon 0%Z);
                   blk_phis := [];
-                  blk_code := [(IId (Name "r"), (INSTR_Op (OP_IBinop (UDiv false) (TYPE_I 64%Z) EXP_Undef (EXP_Integer 1%Z))))];
-                  blk_term := (IVoid 0%Z, TERM_Ret ((TYPE_I 64%Z), (EXP_Ident (ID_Local (Name "r")))));
+                  blk_code := [(IId (Name "r"), (INSTR_Op (OP_IBinop (UDiv false) (TYPE_I 64%N) EXP_Undef (EXP_Integer 1%Z))))];
+                  blk_term := TERM_Ret ((TYPE_I 64%N), (EXP_Ident (ID_Local (Name "r"))));
                   blk_comments := None
                 |}]
                 |}; 
 TLE_Definition {|
   df_prototype := {|dc_name := (Name "test8");
-                    dc_type := (TYPE_Function (TYPE_I 64%Z) []);
+                    dc_type := (TYPE_Function (TYPE_I 64%N) []);
                     dc_param_attrs := ([], []);
                     dc_linkage := None;
                     dc_visibility := None;
@@ -1764,14 +1764,14 @@ TLE_Definition {|
                 {|
                   blk_id := (Anon 0%Z);
                   blk_phis := [];
-                  blk_code := [(IId (Name "r"), (INSTR_Op (OP_IBinop (SDiv false) (TYPE_I 64%Z) EXP_Undef (EXP_Integer 1%Z))))];
-                  blk_term := (IVoid 0%Z, TERM_Ret ((TYPE_I 64%Z), (EXP_Ident (ID_Local (Name "r")))));
+                  blk_code := [(IId (Name "r"), (INSTR_Op (OP_IBinop (SDiv false) (TYPE_I 64%N) EXP_Undef (EXP_Integer 1%Z))))];
+                  blk_term := TERM_Ret ((TYPE_I 64%N), (EXP_Ident (ID_Local (Name "r"))));
                   blk_comments := None
                 |}]
                 |}; 
 TLE_Definition {|
   df_prototype := {|dc_name := (Name "test9");
-                    dc_type := (TYPE_Function (TYPE_I 64%Z) []);
+                    dc_type := (TYPE_Function (TYPE_I 64%N) []);
                     dc_param_attrs := ([], []);
                     dc_linkage := None;
                     dc_visibility := None;
@@ -1786,14 +1786,14 @@ TLE_Definition {|
                 {|
                   blk_id := (Anon 0%Z);
                   blk_phis := [];
-                  blk_code := [(IId (Name "r"), (INSTR_Op (OP_IBinop URem (TYPE_I 64%Z) EXP_Undef (EXP_Integer 1%Z))))];
-                  blk_term := (IVoid 0%Z, TERM_Ret ((TYPE_I 64%Z), (EXP_Ident (ID_Local (Name "r")))));
+                  blk_code := [(IId (Name "r"), (INSTR_Op (OP_IBinop URem (TYPE_I 64%N) EXP_Undef (EXP_Integer 1%Z))))];
+                  blk_term := TERM_Ret ((TYPE_I 64%N), (EXP_Ident (ID_Local (Name "r"))));
                   blk_comments := None
                 |}]
                 |}; 
 TLE_Definition {|
   df_prototype := {|dc_name := (Name "test10");
-                    dc_type := (TYPE_Function (TYPE_I 64%Z) []);
+                    dc_type := (TYPE_Function (TYPE_I 64%N) []);
                     dc_param_attrs := ([], []);
                     dc_linkage := None;
                     dc_visibility := None;
@@ -1808,14 +1808,14 @@ TLE_Definition {|
                 {|
                   blk_id := (Anon 0%Z);
                   blk_phis := [];
-                  blk_code := [(IId (Name "r"), (INSTR_Op (OP_IBinop SRem (TYPE_I 64%Z) EXP_Undef (EXP_Integer 1%Z))))];
-                  blk_term := (IVoid 0%Z, TERM_Ret ((TYPE_I 64%Z), (EXP_Ident (ID_Local (Name "r")))));
+                  blk_code := [(IId (Name "r"), (INSTR_Op (OP_IBinop SRem (TYPE_I 64%N) EXP_Undef (EXP_Integer 1%Z))))];
+                  blk_term := TERM_Ret ((TYPE_I 64%N), (EXP_Ident (ID_Local (Name "r"))));
                   blk_comments := None
                 |}]
                 |}; 
 TLE_Definition {|
   df_prototype := {|dc_name := (Name "test11");
-                    dc_type := (TYPE_Function (TYPE_I 64%Z) []);
+                    dc_type := (TYPE_Function (TYPE_I 64%N) []);
                     dc_param_attrs := ([], []);
                     dc_linkage := None;
                     dc_visibility := None;
@@ -1830,14 +1830,14 @@ TLE_Definition {|
                 {|
                   blk_id := (Anon 0%Z);
                   blk_phis := [];
-                  blk_code := [(IId (Name "r"), (INSTR_Op (OP_IBinop (Shl false false) (TYPE_I 64%Z) EXP_Undef EXP_Undef)))];
-                  blk_term := (IVoid 0%Z, TERM_Ret ((TYPE_I 64%Z), (EXP_Ident (ID_Local (Name "r")))));
+                  blk_code := [(IId (Name "r"), (INSTR_Op (OP_IBinop (Shl false false) (TYPE_I 64%N) EXP_Undef EXP_Undef)))];
+                  blk_term := TERM_Ret ((TYPE_I 64%N), (EXP_Ident (ID_Local (Name "r"))));
                   blk_comments := None
                 |}]
                 |}; 
 TLE_Definition {|
   df_prototype := {|dc_name := (Name "test11b");
-                    dc_type := (TYPE_Function (TYPE_I 64%Z) [(TYPE_I 64%Z)]);
+                    dc_type := (TYPE_Function (TYPE_I 64%N) [(TYPE_I 64%N)]);
                     dc_param_attrs := ([], []);
                     dc_linkage := None;
                     dc_visibility := None;
@@ -1852,14 +1852,14 @@ TLE_Definition {|
                 {|
                   blk_id := (Anon 0%Z);
                   blk_phis := [];
-                  blk_code := [(IId (Name "r"), (INSTR_Op (OP_IBinop (Shl false false) (TYPE_I 64%Z) (EXP_Ident (ID_Local (Name "a"))) EXP_Undef)))];
-                  blk_term := (IVoid 0%Z, TERM_Ret ((TYPE_I 64%Z), (EXP_Ident (ID_Local (Name "r")))));
+                  blk_code := [(IId (Name "r"), (INSTR_Op (OP_IBinop (Shl false false) (TYPE_I 64%N) (EXP_Ident (ID_Local (Name "a"))) EXP_Undef)))];
+                  blk_term := TERM_Ret ((TYPE_I 64%N), (EXP_Ident (ID_Local (Name "r"))));
                   blk_comments := None
                 |}]
                 |}; 
 TLE_Definition {|
   df_prototype := {|dc_name := (Name "test12");
-                    dc_type := (TYPE_Function (TYPE_I 64%Z) []);
+                    dc_type := (TYPE_Function (TYPE_I 64%N) []);
                     dc_param_attrs := ([], []);
                     dc_linkage := None;
                     dc_visibility := None;
@@ -1874,14 +1874,14 @@ TLE_Definition {|
                 {|
                   blk_id := (Anon 0%Z);
                   blk_phis := [];
-                  blk_code := [(IId (Name "r"), (INSTR_Op (OP_IBinop (AShr false) (TYPE_I 64%Z) EXP_Undef EXP_Undef)))];
-                  blk_term := (IVoid 0%Z, TERM_Ret ((TYPE_I 64%Z), (EXP_Ident (ID_Local (Name "r")))));
+                  blk_code := [(IId (Name "r"), (INSTR_Op (OP_IBinop (AShr false) (TYPE_I 64%N) EXP_Undef EXP_Undef)))];
+                  blk_term := TERM_Ret ((TYPE_I 64%N), (EXP_Ident (ID_Local (Name "r"))));
                   blk_comments := None
                 |}]
                 |}; 
 TLE_Definition {|
   df_prototype := {|dc_name := (Name "test12b");
-                    dc_type := (TYPE_Function (TYPE_I 64%Z) [(TYPE_I 64%Z)]);
+                    dc_type := (TYPE_Function (TYPE_I 64%N) [(TYPE_I 64%N)]);
                     dc_param_attrs := ([], []);
                     dc_linkage := None;
                     dc_visibility := None;
@@ -1896,14 +1896,14 @@ TLE_Definition {|
                 {|
                   blk_id := (Anon 0%Z);
                   blk_phis := [];
-                  blk_code := [(IId (Name "r"), (INSTR_Op (OP_IBinop (AShr false) (TYPE_I 64%Z) (EXP_Ident (ID_Local (Name "a"))) EXP_Undef)))];
-                  blk_term := (IVoid 0%Z, TERM_Ret ((TYPE_I 64%Z), (EXP_Ident (ID_Local (Name "r")))));
+                  blk_code := [(IId (Name "r"), (INSTR_Op (OP_IBinop (AShr false) (TYPE_I 64%N) (EXP_Ident (ID_Local (Name "a"))) EXP_Undef)))];
+                  blk_term := TERM_Ret ((TYPE_I 64%N), (EXP_Ident (ID_Local (Name "r"))));
                   blk_comments := None
                 |}]
                 |}; 
 TLE_Definition {|
   df_prototype := {|dc_name := (Name "test13");
-                    dc_type := (TYPE_Function (TYPE_I 64%Z) []);
+                    dc_type := (TYPE_Function (TYPE_I 64%N) []);
                     dc_param_attrs := ([], []);
                     dc_linkage := None;
                     dc_visibility := None;
@@ -1918,14 +1918,14 @@ TLE_Definition {|
                 {|
                   blk_id := (Anon 0%Z);
                   blk_phis := [];
-                  blk_code := [(IId (Name "r"), (INSTR_Op (OP_IBinop (LShr false) (TYPE_I 64%Z) EXP_Undef EXP_Undef)))];
-                  blk_term := (IVoid 0%Z, TERM_Ret ((TYPE_I 64%Z), (EXP_Ident (ID_Local (Name "r")))));
+                  blk_code := [(IId (Name "r"), (INSTR_Op (OP_IBinop (LShr false) (TYPE_I 64%N) EXP_Undef EXP_Undef)))];
+                  blk_term := TERM_Ret ((TYPE_I 64%N), (EXP_Ident (ID_Local (Name "r"))));
                   blk_comments := None
                 |}]
                 |}; 
 TLE_Definition {|
   df_prototype := {|dc_name := (Name "test13b");
-                    dc_type := (TYPE_Function (TYPE_I 64%Z) [(TYPE_I 64%Z)]);
+                    dc_type := (TYPE_Function (TYPE_I 64%N) [(TYPE_I 64%N)]);
                     dc_param_attrs := ([], []);
                     dc_linkage := None;
                     dc_visibility := None;
@@ -1940,14 +1940,14 @@ TLE_Definition {|
                 {|
                   blk_id := (Anon 0%Z);
                   blk_phis := [];
-                  blk_code := [(IId (Name "r"), (INSTR_Op (OP_IBinop (LShr false) (TYPE_I 64%Z) (EXP_Ident (ID_Local (Name "a"))) EXP_Undef)))];
-                  blk_term := (IVoid 0%Z, TERM_Ret ((TYPE_I 64%Z), (EXP_Ident (ID_Local (Name "r")))));
+                  blk_code := [(IId (Name "r"), (INSTR_Op (OP_IBinop (LShr false) (TYPE_I 64%N) (EXP_Ident (ID_Local (Name "a"))) EXP_Undef)))];
+                  blk_term := TERM_Ret ((TYPE_I 64%N), (EXP_Ident (ID_Local (Name "r"))));
                   blk_comments := None
                 |}]
                 |}; 
 TLE_Definition {|
   df_prototype := {|dc_name := (Name "test14");
-                    dc_type := (TYPE_Function (TYPE_I 1%Z) []);
+                    dc_type := (TYPE_Function (TYPE_I 1%N) []);
                     dc_param_attrs := ([], []);
                     dc_linkage := None;
                     dc_visibility := None;
@@ -1962,14 +1962,14 @@ TLE_Definition {|
                 {|
                   blk_id := (Anon 0%Z);
                   blk_phis := [];
-                  blk_code := [(IId (Name "r"), (INSTR_Op (OP_ICmp Slt (TYPE_I 64%Z) EXP_Undef EXP_Undef)))];
-                  blk_term := (IVoid 0%Z, TERM_Ret ((TYPE_I 1%Z), (EXP_Ident (ID_Local (Name "r")))));
+                  blk_code := [(IId (Name "r"), (INSTR_Op (OP_ICmp Slt (TYPE_I 64%N) EXP_Undef EXP_Undef)))];
+                  blk_term := TERM_Ret ((TYPE_I 1%N), (EXP_Ident (ID_Local (Name "r"))));
                   blk_comments := None
                 |}]
                 |}; 
 TLE_Definition {|
   df_prototype := {|dc_name := (Name "test15");
-                    dc_type := (TYPE_Function (TYPE_I 1%Z) []);
+                    dc_type := (TYPE_Function (TYPE_I 1%N) []);
                     dc_param_attrs := ([], []);
                     dc_linkage := None;
                     dc_visibility := None;
@@ -1984,14 +1984,14 @@ TLE_Definition {|
                 {|
                   blk_id := (Anon 0%Z);
                   blk_phis := [];
-                  blk_code := [(IId (Name "r"), (INSTR_Op (OP_ICmp Ult (TYPE_I 64%Z) EXP_Undef EXP_Undef)))];
-                  blk_term := (IVoid 0%Z, TERM_Ret ((TYPE_I 1%Z), (EXP_Ident (ID_Local (Name "r")))));
+                  blk_code := [(IId (Name "r"), (INSTR_Op (OP_ICmp Ult (TYPE_I 64%N) EXP_Undef EXP_Undef)))];
+                  blk_term := TERM_Ret ((TYPE_I 1%N), (EXP_Ident (ID_Local (Name "r"))));
                   blk_comments := None
                 |}]
                 |}; 
 TLE_Definition {|
   df_prototype := {|dc_name := (Name "test16");
-                    dc_type := (TYPE_Function (TYPE_I 64%Z) [(TYPE_I 64%Z)]);
+                    dc_type := (TYPE_Function (TYPE_I 64%N) [(TYPE_I 64%N)]);
                     dc_param_attrs := ([], []);
                     dc_linkage := None;
                     dc_visibility := None;
@@ -2006,14 +2006,14 @@ TLE_Definition {|
                 {|
                   blk_id := (Anon 0%Z);
                   blk_phis := [];
-                  blk_code := [(IId (Name "r"), (INSTR_Op (OP_Select ((TYPE_I 1%Z),EXP_Undef) ((TYPE_I 64%Z),(EXP_Ident (ID_Local (Name "a")))) ((TYPE_I 64%Z),EXP_Undef))))];
-                  blk_term := (IVoid 0%Z, TERM_Ret ((TYPE_I 64%Z), (EXP_Ident (ID_Local (Name "r")))));
+                  blk_code := [(IId (Name "r"), (INSTR_Op (OP_Select ((TYPE_I 1%N),EXP_Undef) ((TYPE_I 64%N),(EXP_Ident (ID_Local (Name "a")))) ((TYPE_I 64%N),EXP_Undef))))];
+                  blk_term := TERM_Ret ((TYPE_I 64%N), (EXP_Ident (ID_Local (Name "r"))));
                   blk_comments := None
                 |}]
                 |}; 
 TLE_Definition {|
   df_prototype := {|dc_name := (Name "test17");
-                    dc_type := (TYPE_Function (TYPE_I 64%Z) [(TYPE_I 64%Z)]);
+                    dc_type := (TYPE_Function (TYPE_I 64%N) [(TYPE_I 64%N)]);
                     dc_param_attrs := ([], []);
                     dc_linkage := None;
                     dc_visibility := None;
@@ -2028,14 +2028,14 @@ TLE_Definition {|
                 {|
                   blk_id := (Anon 0%Z);
                   blk_phis := [];
-                  blk_code := [(IId (Name "r"), (INSTR_Op (OP_Select ((TYPE_I 1%Z),EXP_Undef) ((TYPE_I 64%Z),EXP_Undef) ((TYPE_I 64%Z),(EXP_Ident (ID_Local (Name "a")))))))];
-                  blk_term := (IVoid 0%Z, TERM_Ret ((TYPE_I 64%Z), (EXP_Ident (ID_Local (Name "r")))));
+                  blk_code := [(IId (Name "r"), (INSTR_Op (OP_Select ((TYPE_I 1%N),EXP_Undef) ((TYPE_I 64%N),EXP_Undef) ((TYPE_I 64%N),(EXP_Ident (ID_Local (Name "a")))))))];
+                  blk_term := TERM_Ret ((TYPE_I 64%N), (EXP_Ident (ID_Local (Name "r"))));
                   blk_comments := None
                 |}]
                 |}; 
 TLE_Definition {|
   df_prototype := {|dc_name := (Name "test18");
-                    dc_type := (TYPE_Function (TYPE_I 64%Z) [(TYPE_I 64%Z)]);
+                    dc_type := (TYPE_Function (TYPE_I 64%N) [(TYPE_I 64%N)]);
                     dc_param_attrs := ([], []);
                     dc_linkage := None;
                     dc_visibility := None;
@@ -2050,14 +2050,14 @@ TLE_Definition {|
                 {|
                   blk_id := (Anon 0%Z);
                   blk_phis := [];
-                  blk_code := [(IId (Name "r"), (INSTR_Call ((TYPE_Function (TYPE_I 64%Z) [(TYPE_I 64%Z)]), EXP_Undef) [((TYPE_I 64%Z), (EXP_Ident (ID_Local (Name "a"))))]))];
-                  blk_term := (IVoid 0%Z, TERM_Ret ((TYPE_I 64%Z), (EXP_Ident (ID_Local (Name "r")))));
+                  blk_code := [(IId (Name "r"), (INSTR_Call ((TYPE_Function (TYPE_I 64%N) [(TYPE_I 64%N)]), EXP_Undef) [((TYPE_I 64%N), (EXP_Ident (ID_Local (Name "a"))))]))];
+                  blk_term := TERM_Ret ((TYPE_I 64%N), (EXP_Ident (ID_Local (Name "r"))));
                   blk_comments := None
                 |}]
                 |}; 
 TLE_Definition {|
   df_prototype := {|dc_name := (Name "test19");
-                    dc_type := (TYPE_Function (TYPE_Vector 4%Z (TYPE_I 8%Z)) [(TYPE_Vector 4%Z (TYPE_I 8%Z))]);
+                    dc_type := (TYPE_Function (TYPE_Vector 4%N (TYPE_I 8%N)) [(TYPE_Vector 4%N (TYPE_I 8%N))]);
                     dc_param_attrs := ([], []);
                     dc_linkage := None;
                     dc_visibility := None;
@@ -2072,14 +2072,14 @@ TLE_Definition {|
                 {|
                   blk_id := (Anon 0%Z);
                   blk_phis := [];
-                  blk_code := [(IId (Name "b"), (INSTR_Op (OP_IBinop (Shl false false) (TYPE_Vector 4%Z (TYPE_I 8%Z)) (EXP_Ident (ID_Local (Name "a"))) (EXP_Vector [((TYPE_I 8%Z),(EXP_Integer 8%Z)); ((TYPE_I 8%Z),(EXP_Integer 9%Z)); ((TYPE_I 8%Z),EXP_Undef); ((TYPE_I 8%Z), (EXP_Integer (-1)%Z))]))))];
-                  blk_term := (IVoid 0%Z, TERM_Ret ((TYPE_Vector 4%Z (TYPE_I 8%Z)), (EXP_Ident (ID_Local (Name "b")))));
+                  blk_code := [(IId (Name "b"), (INSTR_Op (OP_IBinop (Shl false false) (TYPE_Vector 4%N (TYPE_I 8%N)) (EXP_Ident (ID_Local (Name "a"))) (EXP_Vector [((TYPE_I 8%N),(EXP_Integer 8%Z)); ((TYPE_I 8%N),(EXP_Integer 9%Z)); ((TYPE_I 8%N),EXP_Undef); ((TYPE_I 8%N), (EXP_Integer (-1)%Z))]))))];
+                  blk_term := TERM_Ret ((TYPE_Vector 4%N (TYPE_I 8%N)), (EXP_Ident (ID_Local (Name "b"))));
                   blk_comments := None
                 |}]
                 |}; 
 TLE_Definition {|
   df_prototype := {|dc_name := (Name "test20");
-                    dc_type := (TYPE_Function (TYPE_I 32%Z) [(TYPE_I 32%Z)]);
+                    dc_type := (TYPE_Function (TYPE_I 32%N) [(TYPE_I 32%N)]);
                     dc_param_attrs := ([], []);
                     dc_linkage := None;
                     dc_visibility := None;
@@ -2094,14 +2094,14 @@ TLE_Definition {|
                 {|
                   blk_id := (Anon 0%Z);
                   blk_phis := [];
-                  blk_code := [(IId (Name "b"), (INSTR_Op (OP_IBinop (UDiv false) (TYPE_I 32%Z) (EXP_Ident (ID_Local (Name "a"))) (EXP_Integer 0%Z))))];
-                  blk_term := (IVoid 0%Z, TERM_Ret ((TYPE_I 32%Z), (EXP_Ident (ID_Local (Name "b")))));
+                  blk_code := [(IId (Name "b"), (INSTR_Op (OP_IBinop (UDiv false) (TYPE_I 32%N) (EXP_Ident (ID_Local (Name "a"))) (EXP_Integer 0%Z))))];
+                  blk_term := TERM_Ret ((TYPE_I 32%N), (EXP_Ident (ID_Local (Name "b"))));
                   blk_comments := None
                 |}]
                 |}; 
 TLE_Definition {|
   df_prototype := {|dc_name := (Name "test20vec");
-                    dc_type := (TYPE_Function (TYPE_Vector 2%Z (TYPE_I 32%Z)) [(TYPE_Vector 2%Z (TYPE_I 32%Z))]);
+                    dc_type := (TYPE_Function (TYPE_Vector 2%N (TYPE_I 32%N)) [(TYPE_Vector 2%N (TYPE_I 32%N))]);
                     dc_param_attrs := ([], []);
                     dc_linkage := None;
                     dc_visibility := None;
@@ -2116,14 +2116,14 @@ TLE_Definition {|
                 {|
                   blk_id := (Anon 0%Z);
                   blk_phis := [];
-                  blk_code := [(IId (Name "b"), (INSTR_Op (OP_IBinop (UDiv false) (TYPE_Vector 2%Z (TYPE_I 32%Z)) (EXP_Ident (ID_Local (Name "a"))) EXP_Zero_initializer)))];
-                  blk_term := (IVoid 0%Z, TERM_Ret ((TYPE_Vector 2%Z (TYPE_I 32%Z)), (EXP_Ident (ID_Local (Name "b")))));
+                  blk_code := [(IId (Name "b"), (INSTR_Op (OP_IBinop (UDiv false) (TYPE_Vector 2%N (TYPE_I 32%N)) (EXP_Ident (ID_Local (Name "a"))) EXP_Zero_initializer)))];
+                  blk_term := TERM_Ret ((TYPE_Vector 2%N (TYPE_I 32%N)), (EXP_Ident (ID_Local (Name "b"))));
                   blk_comments := None
                 |}]
                 |}; 
 TLE_Definition {|
   df_prototype := {|dc_name := (Name "test21");
-                    dc_type := (TYPE_Function (TYPE_I 32%Z) [(TYPE_I 32%Z)]);
+                    dc_type := (TYPE_Function (TYPE_I 32%N) [(TYPE_I 32%N)]);
                     dc_param_attrs := ([], []);
                     dc_linkage := None;
                     dc_visibility := None;
@@ -2138,14 +2138,14 @@ TLE_Definition {|
                 {|
                   blk_id := (Anon 0%Z);
                   blk_phis := [];
-                  blk_code := [(IId (Name "b"), (INSTR_Op (OP_IBinop (SDiv false) (TYPE_I 32%Z) (EXP_Ident (ID_Local (Name "a"))) (EXP_Integer 0%Z))))];
-                  blk_term := (IVoid 0%Z, TERM_Ret ((TYPE_I 32%Z), (EXP_Ident (ID_Local (Name "b")))));
+                  blk_code := [(IId (Name "b"), (INSTR_Op (OP_IBinop (SDiv false) (TYPE_I 32%N) (EXP_Ident (ID_Local (Name "a"))) (EXP_Integer 0%Z))))];
+                  blk_term := TERM_Ret ((TYPE_I 32%N), (EXP_Ident (ID_Local (Name "b"))));
                   blk_comments := None
                 |}]
                 |}; 
 TLE_Definition {|
   df_prototype := {|dc_name := (Name "test21vec");
-                    dc_type := (TYPE_Function (TYPE_Vector 2%Z (TYPE_I 32%Z)) [(TYPE_Vector 2%Z (TYPE_I 32%Z))]);
+                    dc_type := (TYPE_Function (TYPE_Vector 2%N (TYPE_I 32%N)) [(TYPE_Vector 2%N (TYPE_I 32%N))]);
                     dc_param_attrs := ([], []);
                     dc_linkage := None;
                     dc_visibility := None;
@@ -2160,14 +2160,14 @@ TLE_Definition {|
                 {|
                   blk_id := (Anon 0%Z);
                   blk_phis := [];
-                  blk_code := [(IId (Name "b"), (INSTR_Op (OP_IBinop (SDiv false) (TYPE_Vector 2%Z (TYPE_I 32%Z)) (EXP_Ident (ID_Local (Name "a"))) EXP_Zero_initializer)))];
-                  blk_term := (IVoid 0%Z, TERM_Ret ((TYPE_Vector 2%Z (TYPE_I 32%Z)), (EXP_Ident (ID_Local (Name "b")))));
+                  blk_code := [(IId (Name "b"), (INSTR_Op (OP_IBinop (SDiv false) (TYPE_Vector 2%N (TYPE_I 32%N)) (EXP_Ident (ID_Local (Name "a"))) EXP_Zero_initializer)))];
+                  blk_term := TERM_Ret ((TYPE_Vector 2%N (TYPE_I 32%N)), (EXP_Ident (ID_Local (Name "b"))));
                   blk_comments := None
                 |}]
                 |}; 
 TLE_Definition {|
   df_prototype := {|dc_name := (Name "test22");
-                    dc_type := (TYPE_Function (TYPE_I 32%Z) [(TYPE_I 32%Z)]);
+                    dc_type := (TYPE_Function (TYPE_I 32%N) [(TYPE_I 32%N)]);
                     dc_param_attrs := ([], []);
                     dc_linkage := None;
                     dc_visibility := None;
@@ -2182,14 +2182,14 @@ TLE_Definition {|
                 {|
                   blk_id := (Anon 0%Z);
                   blk_phis := [];
-                  blk_code := [(IId (Name "b"), (INSTR_Op (OP_IBinop (AShr true) (TYPE_I 32%Z) EXP_Undef (EXP_Ident (ID_Local (Name "a"))))))];
-                  blk_term := (IVoid 0%Z, TERM_Ret ((TYPE_I 32%Z), (EXP_Ident (ID_Local (Name "b")))));
+                  blk_code := [(IId (Name "b"), (INSTR_Op (OP_IBinop (AShr true) (TYPE_I 32%N) EXP_Undef (EXP_Ident (ID_Local (Name "a"))))))];
+                  blk_term := TERM_Ret ((TYPE_I 32%N), (EXP_Ident (ID_Local (Name "b"))));
                   blk_comments := None
                 |}]
                 |}; 
 TLE_Definition {|
   df_prototype := {|dc_name := (Name "test23");
-                    dc_type := (TYPE_Function (TYPE_I 32%Z) [(TYPE_I 32%Z)]);
+                    dc_type := (TYPE_Function (TYPE_I 32%N) [(TYPE_I 32%N)]);
                     dc_param_attrs := ([], []);
                     dc_linkage := None;
                     dc_visibility := None;
@@ -2204,14 +2204,14 @@ TLE_Definition {|
                 {|
                   blk_id := (Anon 0%Z);
                   blk_phis := [];
-                  blk_code := [(IId (Name "b"), (INSTR_Op (OP_IBinop (LShr true) (TYPE_I 32%Z) EXP_Undef (EXP_Ident (ID_Local (Name "a"))))))];
-                  blk_term := (IVoid 0%Z, TERM_Ret ((TYPE_I 32%Z), (EXP_Ident (ID_Local (Name "b")))));
+                  blk_code := [(IId (Name "b"), (INSTR_Op (OP_IBinop (LShr true) (TYPE_I 32%N) EXP_Undef (EXP_Ident (ID_Local (Name "a"))))))];
+                  blk_term := TERM_Ret ((TYPE_I 32%N), (EXP_Ident (ID_Local (Name "b"))));
                   blk_comments := None
                 |}]
                 |}; 
 TLE_Definition {|
   df_prototype := {|dc_name := (Name "test24");
-                    dc_type := (TYPE_Function (TYPE_I 32%Z) []);
+                    dc_type := (TYPE_Function (TYPE_I 32%N) []);
                     dc_param_attrs := ([], []);
                     dc_linkage := None;
                     dc_visibility := None;
@@ -2226,14 +2226,14 @@ TLE_Definition {|
                 {|
                   blk_id := (Anon 0%Z);
                   blk_phis := [];
-                  blk_code := [(IId (Name "b"), (INSTR_Op (OP_IBinop (UDiv false) (TYPE_I 32%Z) EXP_Undef (EXP_Integer 0%Z))))];
-                  blk_term := (IVoid 0%Z, TERM_Ret ((TYPE_I 32%Z), (EXP_Ident (ID_Local (Name "b")))));
+                  blk_code := [(IId (Name "b"), (INSTR_Op (OP_IBinop (UDiv false) (TYPE_I 32%N) EXP_Undef (EXP_Integer 0%Z))))];
+                  blk_term := TERM_Ret ((TYPE_I 32%N), (EXP_Ident (ID_Local (Name "b"))));
                   blk_comments := None
                 |}]
                 |}; 
 TLE_Definition {|
   df_prototype := {|dc_name := (Name "test25");
-                    dc_type := (TYPE_Function (TYPE_I 32%Z) []);
+                    dc_type := (TYPE_Function (TYPE_I 32%N) []);
                     dc_param_attrs := ([], []);
                     dc_linkage := None;
                     dc_visibility := None;
@@ -2248,14 +2248,14 @@ TLE_Definition {|
                 {|
                   blk_id := (Anon 0%Z);
                   blk_phis := [];
-                  blk_code := [(IId (Name "b"), (INSTR_Op (OP_IBinop (LShr false) (TYPE_I 32%Z) (EXP_Integer 0%Z) EXP_Undef)))];
-                  blk_term := (IVoid 0%Z, TERM_Ret ((TYPE_I 32%Z), (EXP_Ident (ID_Local (Name "b")))));
+                  blk_code := [(IId (Name "b"), (INSTR_Op (OP_IBinop (LShr false) (TYPE_I 32%N) (EXP_Integer 0%Z) EXP_Undef)))];
+                  blk_term := TERM_Ret ((TYPE_I 32%N), (EXP_Ident (ID_Local (Name "b"))));
                   blk_comments := None
                 |}]
                 |}; 
 TLE_Definition {|
   df_prototype := {|dc_name := (Name "test26");
-                    dc_type := (TYPE_Function (TYPE_I 32%Z) []);
+                    dc_type := (TYPE_Function (TYPE_I 32%N) []);
                     dc_param_attrs := ([], []);
                     dc_linkage := None;
                     dc_visibility := None;
@@ -2270,14 +2270,14 @@ TLE_Definition {|
                 {|
                   blk_id := (Anon 0%Z);
                   blk_phis := [];
-                  blk_code := [(IId (Name "b"), (INSTR_Op (OP_IBinop (AShr false) (TYPE_I 32%Z) (EXP_Integer 0%Z) EXP_Undef)))];
-                  blk_term := (IVoid 0%Z, TERM_Ret ((TYPE_I 32%Z), (EXP_Ident (ID_Local (Name "b")))));
+                  blk_code := [(IId (Name "b"), (INSTR_Op (OP_IBinop (AShr false) (TYPE_I 32%N) (EXP_Integer 0%Z) EXP_Undef)))];
+                  blk_term := TERM_Ret ((TYPE_I 32%N), (EXP_Ident (ID_Local (Name "b"))));
                   blk_comments := None
                 |}]
                 |}; 
 TLE_Definition {|
   df_prototype := {|dc_name := (Name "test27");
-                    dc_type := (TYPE_Function (TYPE_I 32%Z) []);
+                    dc_type := (TYPE_Function (TYPE_I 32%N) []);
                     dc_param_attrs := ([], []);
                     dc_linkage := None;
                     dc_visibility := None;
@@ -2292,14 +2292,14 @@ TLE_Definition {|
                 {|
                   blk_id := (Anon 0%Z);
                   blk_phis := [];
-                  blk_code := [(IId (Name "b"), (INSTR_Op (OP_IBinop (Shl false false) (TYPE_I 32%Z) (EXP_Integer 0%Z) EXP_Undef)))];
-                  blk_term := (IVoid 0%Z, TERM_Ret ((TYPE_I 32%Z), (EXP_Ident (ID_Local (Name "b")))));
+                  blk_code := [(IId (Name "b"), (INSTR_Op (OP_IBinop (Shl false false) (TYPE_I 32%N) (EXP_Integer 0%Z) EXP_Undef)))];
+                  blk_term := TERM_Ret ((TYPE_I 32%N), (EXP_Ident (ID_Local (Name "b"))));
                   blk_comments := None
                 |}]
                 |}; 
 TLE_Definition {|
   df_prototype := {|dc_name := (Name "test28");
-                    dc_type := (TYPE_Function (TYPE_I 32%Z) [(TYPE_I 32%Z)]);
+                    dc_type := (TYPE_Function (TYPE_I 32%N) [(TYPE_I 32%N)]);
                     dc_param_attrs := ([], []);
                     dc_linkage := None;
                     dc_visibility := None;
@@ -2314,14 +2314,14 @@ TLE_Definition {|
                 {|
                   blk_id := (Anon 0%Z);
                   blk_phis := [];
-                  blk_code := [(IId (Name "b"), (INSTR_Op (OP_IBinop (Shl false true) (TYPE_I 32%Z) EXP_Undef (EXP_Ident (ID_Local (Name "a"))))))];
-                  blk_term := (IVoid 0%Z, TERM_Ret ((TYPE_I 32%Z), (EXP_Ident (ID_Local (Name "b")))));
+                  blk_code := [(IId (Name "b"), (INSTR_Op (OP_IBinop (Shl false true) (TYPE_I 32%N) EXP_Undef (EXP_Ident (ID_Local (Name "a"))))))];
+                  blk_term := TERM_Ret ((TYPE_I 32%N), (EXP_Ident (ID_Local (Name "b"))));
                   blk_comments := None
                 |}]
                 |}; 
 TLE_Definition {|
   df_prototype := {|dc_name := (Name "test29");
-                    dc_type := (TYPE_Function (TYPE_I 32%Z) [(TYPE_I 32%Z)]);
+                    dc_type := (TYPE_Function (TYPE_I 32%N) [(TYPE_I 32%N)]);
                     dc_param_attrs := ([], []);
                     dc_linkage := None;
                     dc_visibility := None;
@@ -2336,14 +2336,14 @@ TLE_Definition {|
                 {|
                   blk_id := (Anon 0%Z);
                   blk_phis := [];
-                  blk_code := [(IId (Name "b"), (INSTR_Op (OP_IBinop (Shl true false) (TYPE_I 32%Z) EXP_Undef (EXP_Ident (ID_Local (Name "a"))))))];
-                  blk_term := (IVoid 0%Z, TERM_Ret ((TYPE_I 32%Z), (EXP_Ident (ID_Local (Name "b")))));
+                  blk_code := [(IId (Name "b"), (INSTR_Op (OP_IBinop (Shl true false) (TYPE_I 32%N) EXP_Undef (EXP_Ident (ID_Local (Name "a"))))))];
+                  blk_term := TERM_Ret ((TYPE_I 32%N), (EXP_Ident (ID_Local (Name "b"))));
                   blk_comments := None
                 |}]
                 |}; 
 TLE_Definition {|
   df_prototype := {|dc_name := (Name "test30");
-                    dc_type := (TYPE_Function (TYPE_I 32%Z) [(TYPE_I 32%Z)]);
+                    dc_type := (TYPE_Function (TYPE_I 32%N) [(TYPE_I 32%N)]);
                     dc_param_attrs := ([], []);
                     dc_linkage := None;
                     dc_visibility := None;
@@ -2358,14 +2358,14 @@ TLE_Definition {|
                 {|
                   blk_id := (Anon 0%Z);
                   blk_phis := [];
-                  blk_code := [(IId (Name "b"), (INSTR_Op (OP_IBinop (Shl true true) (TYPE_I 32%Z) EXP_Undef (EXP_Ident (ID_Local (Name "a"))))))];
-                  blk_term := (IVoid 0%Z, TERM_Ret ((TYPE_I 32%Z), (EXP_Ident (ID_Local (Name "b")))));
+                  blk_code := [(IId (Name "b"), (INSTR_Op (OP_IBinop (Shl true true) (TYPE_I 32%N) EXP_Undef (EXP_Ident (ID_Local (Name "a"))))))];
+                  blk_term := TERM_Ret ((TYPE_I 32%N), (EXP_Ident (ID_Local (Name "b"))));
                   blk_comments := None
                 |}]
                 |}; 
 TLE_Definition {|
   df_prototype := {|dc_name := (Name "test31");
-                    dc_type := (TYPE_Function (TYPE_I 32%Z) [(TYPE_I 32%Z)]);
+                    dc_type := (TYPE_Function (TYPE_I 32%N) [(TYPE_I 32%N)]);
                     dc_param_attrs := ([], []);
                     dc_linkage := None;
                     dc_visibility := None;
@@ -2380,14 +2380,14 @@ TLE_Definition {|
                 {|
                   blk_id := (Anon 0%Z);
                   blk_phis := [];
-                  blk_code := [(IId (Name "b"), (INSTR_Op (OP_IBinop (Shl false false) (TYPE_I 32%Z) EXP_Undef (EXP_Ident (ID_Local (Name "a"))))))];
-                  blk_term := (IVoid 0%Z, TERM_Ret ((TYPE_I 32%Z), (EXP_Ident (ID_Local (Name "b")))));
+                  blk_code := [(IId (Name "b"), (INSTR_Op (OP_IBinop (Shl false false) (TYPE_I 32%N) EXP_Undef (EXP_Ident (ID_Local (Name "a"))))))];
+                  blk_term := TERM_Ret ((TYPE_I 32%N), (EXP_Ident (ID_Local (Name "b"))));
                   blk_comments := None
                 |}]
                 |}; 
 TLE_Definition {|
   df_prototype := {|dc_name := (Name "test32");
-                    dc_type := (TYPE_Function (TYPE_I 32%Z) [(TYPE_I 32%Z)]);
+                    dc_type := (TYPE_Function (TYPE_I 32%N) [(TYPE_I 32%N)]);
                     dc_param_attrs := ([], []);
                     dc_linkage := None;
                     dc_visibility := None;
@@ -2402,14 +2402,14 @@ TLE_Definition {|
                 {|
                   blk_id := (Anon 0%Z);
                   blk_phis := [];
-                  blk_code := [(IId (Name "b"), (INSTR_Op (OP_IBinop (Shl false false) (TYPE_I 32%Z) EXP_Undef (EXP_Integer 0%Z))))];
-                  blk_term := (IVoid 0%Z, TERM_Ret ((TYPE_I 32%Z), (EXP_Ident (ID_Local (Name "b")))));
+                  blk_code := [(IId (Name "b"), (INSTR_Op (OP_IBinop (Shl false false) (TYPE_I 32%N) EXP_Undef (EXP_Integer 0%Z))))];
+                  blk_term := TERM_Ret ((TYPE_I 32%N), (EXP_Ident (ID_Local (Name "b"))));
                   blk_comments := None
                 |}]
                 |}; 
 TLE_Definition {|
   df_prototype := {|dc_name := (Name "test33");
-                    dc_type := (TYPE_Function (TYPE_I 32%Z) [(TYPE_I 32%Z)]);
+                    dc_type := (TYPE_Function (TYPE_I 32%N) [(TYPE_I 32%N)]);
                     dc_param_attrs := ([], []);
                     dc_linkage := None;
                     dc_visibility := None;
@@ -2424,14 +2424,14 @@ TLE_Definition {|
                 {|
                   blk_id := (Anon 0%Z);
                   blk_phis := [];
-                  blk_code := [(IId (Name "b"), (INSTR_Op (OP_IBinop (AShr false) (TYPE_I 32%Z) EXP_Undef (EXP_Integer 0%Z))))];
-                  blk_term := (IVoid 0%Z, TERM_Ret ((TYPE_I 32%Z), (EXP_Ident (ID_Local (Name "b")))));
+                  blk_code := [(IId (Name "b"), (INSTR_Op (OP_IBinop (AShr false) (TYPE_I 32%N) EXP_Undef (EXP_Integer 0%Z))))];
+                  blk_term := TERM_Ret ((TYPE_I 32%N), (EXP_Ident (ID_Local (Name "b"))));
                   blk_comments := None
                 |}]
                 |}; 
 TLE_Definition {|
   df_prototype := {|dc_name := (Name "test34");
-                    dc_type := (TYPE_Function (TYPE_I 32%Z) [(TYPE_I 32%Z)]);
+                    dc_type := (TYPE_Function (TYPE_I 32%N) [(TYPE_I 32%N)]);
                     dc_param_attrs := ([], []);
                     dc_linkage := None;
                     dc_visibility := None;
@@ -2446,14 +2446,14 @@ TLE_Definition {|
                 {|
                   blk_id := (Anon 0%Z);
                   blk_phis := [];
-                  blk_code := [(IId (Name "b"), (INSTR_Op (OP_IBinop (LShr false) (TYPE_I 32%Z) EXP_Undef (EXP_Integer 0%Z))))];
-                  blk_term := (IVoid 0%Z, TERM_Ret ((TYPE_I 32%Z), (EXP_Ident (ID_Local (Name "b")))));
+                  blk_code := [(IId (Name "b"), (INSTR_Op (OP_IBinop (LShr false) (TYPE_I 32%N) EXP_Undef (EXP_Integer 0%Z))))];
+                  blk_term := TERM_Ret ((TYPE_I 32%N), (EXP_Ident (ID_Local (Name "b"))));
                   blk_comments := None
                 |}]
                 |}; 
 TLE_Definition {|
   df_prototype := {|dc_name := (Name "test35");
-                    dc_type := (TYPE_Function (TYPE_I 32%Z) [(TYPE_Vector 4%Z (TYPE_I 32%Z))]);
+                    dc_type := (TYPE_Function (TYPE_I 32%N) [(TYPE_Vector 4%N (TYPE_I 32%N))]);
                     dc_param_attrs := ([], []);
                     dc_linkage := None;
                     dc_visibility := None;
@@ -2468,14 +2468,14 @@ TLE_Definition {|
                 {|
                   blk_id := (Anon 0%Z);
                   blk_phis := [];
-                  blk_code := [(IId (Name "b"), (INSTR_Op (OP_ExtractElement ((TYPE_Vector 4%Z (TYPE_I 32%Z)),(EXP_Ident (ID_Local (Name "V")))) ((TYPE_I 32%Z),(EXP_Integer 4%Z)))))];
-                  blk_term := (IVoid 0%Z, TERM_Ret ((TYPE_I 32%Z), (EXP_Ident (ID_Local (Name "b")))));
+                  blk_code := [(IId (Name "b"), (INSTR_Op (OP_ExtractElement ((TYPE_Vector 4%N (TYPE_I 32%N)),(EXP_Ident (ID_Local (Name "V")))) ((TYPE_I 32%N),(EXP_Integer 4%Z)))))];
+                  blk_term := TERM_Ret ((TYPE_I 32%N), (EXP_Ident (ID_Local (Name "b"))));
                   blk_comments := None
                 |}]
                 |}; 
 TLE_Definition {|
   df_prototype := {|dc_name := (Name "test36");
-                    dc_type := (TYPE_Function (TYPE_I 32%Z) [(TYPE_I 32%Z)]);
+                    dc_type := (TYPE_Function (TYPE_I 32%N) [(TYPE_I 32%N)]);
                     dc_param_attrs := ([], []);
                     dc_linkage := None;
                     dc_visibility := None;
@@ -2490,14 +2490,14 @@ TLE_Definition {|
                 {|
                   blk_id := (Anon 0%Z);
                   blk_phis := [];
-                  blk_code := [(IId (Name "b"), (INSTR_Op (OP_ExtractElement ((TYPE_Vector 4%Z (TYPE_I 32%Z)),EXP_Undef) ((TYPE_I 32%Z),(EXP_Ident (ID_Local (Name "V")))))))];
-                  blk_term := (IVoid 0%Z, TERM_Ret ((TYPE_I 32%Z), (EXP_Ident (ID_Local (Name "b")))));
+                  blk_code := [(IId (Name "b"), (INSTR_Op (OP_ExtractElement ((TYPE_Vector 4%N (TYPE_I 32%N)),EXP_Undef) ((TYPE_I 32%N),(EXP_Ident (ID_Local (Name "V")))))))];
+                  blk_term := TERM_Ret ((TYPE_I 32%N), (EXP_Ident (ID_Local (Name "b"))));
                   blk_comments := None
                 |}]
                 |}; 
 TLE_Definition {|
   df_prototype := {|dc_name := (Name "test37");
-                    dc_type := (TYPE_Function (TYPE_I 32%Z) []);
+                    dc_type := (TYPE_Function (TYPE_I 32%N) []);
                     dc_param_attrs := ([], []);
                     dc_linkage := None;
                     dc_visibility := None;
@@ -2512,14 +2512,14 @@ TLE_Definition {|
                 {|
                   blk_id := (Anon 0%Z);
                   blk_phis := [];
-                  blk_code := [(IId (Name "b"), (INSTR_Op (OP_IBinop (UDiv false) (TYPE_I 32%Z) EXP_Undef EXP_Undef)))];
-                  blk_term := (IVoid 0%Z, TERM_Ret ((TYPE_I 32%Z), (EXP_Ident (ID_Local (Name "b")))));
+                  blk_code := [(IId (Name "b"), (INSTR_Op (OP_IBinop (UDiv false) (TYPE_I 32%N) EXP_Undef EXP_Undef)))];
+                  blk_term := TERM_Ret ((TYPE_I 32%N), (EXP_Ident (ID_Local (Name "b"))));
                   blk_comments := None
                 |}]
                 |}; 
 TLE_Definition {|
   df_prototype := {|dc_name := (Name "test38");
-                    dc_type := (TYPE_Function (TYPE_I 32%Z) [(TYPE_I 32%Z)]);
+                    dc_type := (TYPE_Function (TYPE_I 32%N) [(TYPE_I 32%N)]);
                     dc_param_attrs := ([], []);
                     dc_linkage := None;
                     dc_visibility := None;
@@ -2534,14 +2534,14 @@ TLE_Definition {|
                 {|
                   blk_id := (Anon 0%Z);
                   blk_phis := [];
-                  blk_code := [(IId (Name "b"), (INSTR_Op (OP_IBinop (UDiv false) (TYPE_I 32%Z) (EXP_Ident (ID_Local (Name "a"))) EXP_Undef)))];
-                  blk_term := (IVoid 0%Z, TERM_Ret ((TYPE_I 32%Z), (EXP_Ident (ID_Local (Name "b")))));
+                  blk_code := [(IId (Name "b"), (INSTR_Op (OP_IBinop (UDiv false) (TYPE_I 32%N) (EXP_Ident (ID_Local (Name "a"))) EXP_Undef)))];
+                  blk_term := TERM_Ret ((TYPE_I 32%N), (EXP_Ident (ID_Local (Name "b"))));
                   blk_comments := None
                 |}]
                 |}; 
 TLE_Definition {|
   df_prototype := {|dc_name := (Name "test39");
-                    dc_type := (TYPE_Function (TYPE_I 32%Z) []);
+                    dc_type := (TYPE_Function (TYPE_I 32%N) []);
                     dc_param_attrs := ([], []);
                     dc_linkage := None;
                     dc_visibility := None;
@@ -2556,8 +2556,8 @@ TLE_Definition {|
                 {|
                   blk_id := (Anon 0%Z);
                   blk_phis := [];
-                  blk_code := [(IId (Name "b"), (INSTR_Op (OP_IBinop (UDiv false) (TYPE_I 32%Z) (EXP_Integer 0%Z) EXP_Undef)))];
-                  blk_term := (IVoid 0%Z, TERM_Ret ((TYPE_I 32%Z), (EXP_Ident (ID_Local (Name "b")))));
+                  blk_code := [(IId (Name "b"), (INSTR_Op (OP_IBinop (UDiv false) (TYPE_I 32%N) (EXP_Integer 0%Z) EXP_Undef)))];
+                  blk_term := TERM_Ret ((TYPE_I 32%N), (EXP_Ident (ID_Local (Name "b"))));
                   blk_comments := None
                 |}]
                 |}].
